@prefix : <http://kgrc4si.home.kg/virtualhome2kg/ontology/> .
@prefix ac: <http://kgrc4si.home.kg/virtualhome2kg/ontology/action/> .
@prefix dcterms: <http://purl.org/dc/terms/> .
@prefix ho: <http://www.owl-ontologies.com/VirtualHome.owl#> .
@prefix owl: <http://www.w3.org/2002/07/owl#> .
@prefix rdf: <http://www.w3.org/1999/02/22-rdf-syntax-ns#> .
@prefix rdfs: <http://www.w3.org/2000/01/rdf-schema#> .
@prefix skos: <http://www.w3.org/2004/02/skos/core#> .
@prefix time: <http://www.w3.org/2006/time#> .
@prefix x3do: <https://www.web3d.org/specifications/X3dOntology4.0#> .
@prefix xsd: <http://www.w3.org/2001/XMLSchema#> .

: a owl:Ontology ;
    rdfs:comment """This ontology offers vocabularies for representing activities of daily living (ADL) that can be run in the VirtualHome (http://virtual-home.org/), run-time home situations, objects, and relationships among them.\r
This ontology is an extended version of the HomeOntology (https://github.com/valexande/HomeOntology).""" .

:BROKEN a :StateType,
        owl:NamedIndividual .

:BURNING a :StateType,
        owl:NamedIndividual .

:Back_Porch a owl:Class ;
    rdfs:subClassOf :Room .

:Backyard a owl:Class ;
    rdfs:subClassOf :Room .

:Bathroom a owl:Class ;
    rdfs:subClassOf :Room .

:Bedroom a owl:Class ;
    rdfs:subClassOf :Room .

:CLEAN a :StateType,
        owl:NamedIndividual .

:CLOSED a :StateType,
        owl:NamedIndividual .

:COOKED a :StateType,
        owl:NamedIndividual .

:DIRTY a :StateType,
        owl:NamedIndividual .

:DONE a :StateType,
        owl:NamedIndividual .

:DRUNK a :StateType,
        owl:NamedIndividual .

:DRY a :StateType,
        owl:NamedIndividual .

:Dining_room a owl:Class ;
    rdfs:subClassOf :Room .

:EMPTY a :StateType,
        owl:NamedIndividual .

:EndEvent a owl:Class ;
    rdfs:subClassOf :Event .

:Entrance a owl:Class ;
    rdfs:subClassOf :Room .

:FLUSHED a :StateType,
        owl:NamedIndividual .

:FOLDED a :StateType,
        owl:NamedIndividual .

:FROZEN a :StateType,
        owl:NamedIndividual .

:FULL a :StateType,
        owl:NamedIndividual .

:Family_Altar a owl:Class ;
    rdfs:subClassOf :Room .

:HANGED a :StateType,
        owl:NamedIndividual .

:HURT a :StateType,
        owl:NamedIndividual .

:Home a owl:Class ;
    rdfs:subClassOf :Room .

:Home_office a owl:Class ;
    rdfs:subClassOf :Room .

:Kitchen a owl:Class ;
    rdfs:subClassOf :Room .

:LYING a :StateType,
        owl:NamedIndividual .

:Livingroom a owl:Class ;
    rdfs:subClassOf :Room .

:MELTED a :StateType,
        owl:NamedIndividual .

:OCCUPIED a :StateType,
        owl:NamedIndividual .

:OFF a :StateType,
        owl:NamedIndividual .

:ON a :StateType,
        owl:NamedIndividual .

:OPEN a :StateType,
        owl:NamedIndividual .

:PEELED a :StateType,
        owl:NamedIndividual .

:PERSON a :Attribute,
        owl:NamedIndividual .

:PLUGGED_IN a :StateType,
        owl:NamedIndividual .

:PLUGGED_OUT a :StateType,
        owl:NamedIndividual .

:ROTTEN a :StateType,
        owl:NamedIndividual .

:SHARPENED a :StateType,
        owl:NamedIndividual .

:SHAVED a :StateType,
        owl:NamedIndividual .

:SITTING a :StateType,
        owl:NamedIndividual .

:SLICED a :StateType,
        owl:NamedIndividual .

:SQUEEZED a :StateType,
        owl:NamedIndividual .

:Service_Entrance a owl:Class ;
    rdfs:subClassOf :Room .

:Stairs a owl:Class ;
    rdfs:subClassOf :Room .

:StartEvent a owl:Class ;
    rdfs:subClassOf :Event .

:Toilet a owl:Class ;
    rdfs:subClassOf :Room .

:UNDONE a :StateType,
        owl:NamedIndividual .

:WET a :StateType,
        owl:NamedIndividual .

ac:bend a :Action,
        owl:NamedIndividual .

ac:break a :Action,
        owl:NamedIndividual .

ac:breatheIn a :Action,
        owl:NamedIndividual .

ac:breatheOut a :Action,
        owl:NamedIndividual .

ac:brush a :Action,
        owl:NamedIndividual .

ac:call a :Action,
        owl:NamedIndividual .

ac:carry a :Action,
        owl:NamedIndividual .

ac:climb a :Action,
        owl:NamedIndividual .

ac:climbDown a :Action,
        owl:NamedIndividual .

ac:close a :Action,
        owl:NamedIndividual .

ac:cover a :Action,
        owl:NamedIndividual .

ac:crawl a :Action,
        owl:NamedIndividual .

ac:cut a :Action,
        owl:NamedIndividual .

ac:dance a :Action,
        owl:NamedIndividual .

ac:dial a :Action,
        owl:NamedIndividual .

ac:dive a :Action,
        owl:NamedIndividual .

ac:drop a :Action,
        owl:NamedIndividual .

ac:enter a :Action,
        owl:NamedIndividual .

ac:excrete a :Action,
        owl:NamedIndividual .

ac:find a :Action,
        owl:NamedIndividual .

ac:flush a :Action,
        owl:NamedIndividual .

ac:fold a :Action,
        owl:NamedIndividual .

ac:gargle a :Action,
        owl:NamedIndividual .

ac:grab a :Action,
        owl:NamedIndividual .

ac:greet a :Action,
        owl:NamedIndividual .

ac:hang a :Action,
        owl:NamedIndividual .

ac:hit a :Action,
        owl:NamedIndividual .

ac:insert a :Action,
        owl:NamedIndividual .

ac:jump a :Action,
        owl:NamedIndividual .

ac:kneel a :Action,
        owl:NamedIndividual .

ac:laugh a :Action,
        owl:NamedIndividual .

ac:leave a :Action,
        owl:NamedIndividual .

ac:lie a :Action,
        owl:NamedIndividual .

ac:lift a :Action,
        owl:NamedIndividual .

ac:listen a :Action,
        owl:NamedIndividual .

ac:lookAt a :Action,
        owl:NamedIndividual .

ac:maintain a :Action,
        owl:NamedIndividual .

ac:move a :Action,
        owl:NamedIndividual .

ac:open a :Action,
        owl:NamedIndividual .

ac:pickUp a :Action,
        owl:NamedIndividual .

ac:plugIn a :Action,
        owl:NamedIndividual .

ac:plugOut a :Action,
        owl:NamedIndividual .

ac:pointAt a :Action,
        owl:NamedIndividual .

ac:pour a :Action,
        owl:NamedIndividual .

ac:pull a :Action,
        owl:NamedIndividual .

ac:pullOut a :Action,
        owl:NamedIndividual .

ac:push a :Action,
        owl:NamedIndividual .

ac:put a :Action,
        owl:NamedIndividual .

ac:putIn a :Action,
        owl:NamedIndividual .

ac:putOn a :Action,
        owl:NamedIndividual .

ac:reach a :Action,
        owl:NamedIndividual .

ac:rinse a :Action,
        owl:NamedIndividual .

ac:run a :Action,
        owl:NamedIndividual .

ac:scrub a :Action,
        owl:NamedIndividual .

ac:sew a :Action,
        owl:NamedIndividual .

ac:shake a :Action,
        owl:NamedIndividual .

ac:sing a :Action,
        owl:NamedIndividual .

ac:sit a :Action,
        owl:NamedIndividual .

ac:smell a :Action,
        owl:NamedIndividual .

ac:soak a :Action,
        owl:NamedIndividual .

ac:speak a :Action,
        owl:NamedIndividual .

ac:spit a :Action,
        owl:NamedIndividual .

ac:spread a :Action,
        owl:NamedIndividual .

ac:squat a :Action,
        owl:NamedIndividual .

ac:squeeze a :Action,
        owl:NamedIndividual .

ac:stand a :Action,
        owl:NamedIndividual .

ac:standUp a :Action,
        owl:NamedIndividual .

ac:stir a :Action,
        owl:NamedIndividual .

ac:straddle a :Action,
        owl:NamedIndividual .

ac:stretch a :Action,
        owl:NamedIndividual .

ac:strideOver a :Action,
        owl:NamedIndividual .

ac:sweep a :Action,
        owl:NamedIndividual .

ac:swing a :Action,
        owl:NamedIndividual .

ac:switchOff a :Action,
        owl:NamedIndividual .

ac:switchOn a :Action,
        owl:NamedIndividual .

ac:takeOff a :Action,
        owl:NamedIndividual .

ac:talk a :Action,
        owl:NamedIndividual .

ac:taste a :Action,
        owl:NamedIndividual .

ac:throw a :Action,
        owl:NamedIndividual .

ac:tie a :Action,
        owl:NamedIndividual .

ac:touch a :Action,
        owl:NamedIndividual .

ac:turnTo a :Action,
        owl:NamedIndividual .

ac:twist a :Action,
        owl:NamedIndividual .

ac:type a :Action,
        owl:NamedIndividual .

ac:uncover a :Action,
        owl:NamedIndividual .

ac:unfold a :Action,
        owl:NamedIndividual .

ac:unwrap a :Action,
        owl:NamedIndividual .

ac:vacuum a :Action,
        owl:NamedIndividual .

ac:wait a :Action,
        owl:NamedIndividual .

ac:walk a :Action,
        owl:NamedIndividual .

ac:watch a :Action,
        owl:NamedIndividual .

ac:wipe a :Action,
        owl:NamedIndividual .

ac:wrap a :Action,
        owl:NamedIndividual .

ac:write a :Action,
        owl:NamedIndividual .

:actionNumber a owl:DatatypeProperty ;
    rdfs:domain :Action ;
    rdfs:range xsd:int .

:activity a owl:ObjectProperty ;
    rdfs:domain <http://plod.info/rdf/Episode> ;
    rdfs:range ho:Activity .

:activityNumber a owl:DatatypeProperty ;
    rdfs:domain ho:Activity ;
    rdfs:range xsd:int .

:affords a owl:ObjectProperty ;
    rdfs:domain :Object ;
    rdfs:range :Action .

:agent a owl:ObjectProperty ;
    rdfs:domain :Event ;
    rdfs:range :Character ;
    skos:closeMatch <http://purl.org/NET/c4dm/event.owl#agent> .

:attribute a owl:ObjectProperty ;
    rdfs:domain :Object ;
    rdfs:range :Attribute .

:bbox a owl:ObjectProperty ;
    rdfs:comment "3D bounding box" ;
    rdfs:domain :State ;
    rdfs:range x3do:Shape ;
    owl:inverseOf :isBboxOf .

:between a owl:ObjectProperty ;
    rdfs:comment "used for door object, if door is between kitchen and livingroom, we have edges <door, between, livingroom> and <door, between ,kitchen>" ;
    rdfs:domain x3do:Shape ;
    rdfs:range x3do:Shape ;
    rdfs:subPropertyOf :relatedShape .

:close a owl:ObjectProperty ;
    rdfs:comment "edge <object1, close, object2> denotes that the distance between center of object1 (object2) to the bounding box of object2 (object1) is < 1.5 units (~meters)" ;
    rdfs:domain x3do:Shape ;
    rdfs:range x3do:Shape ;
    rdfs:subPropertyOf :relatedShape .

:clothes a :Attribute,
        owl:NamedIndividual .

:containers a :Attribute,
        owl:NamedIndividual .

:cover_object a :Attribute,
        owl:NamedIndividual .

:cream a :Attribute,
        owl:NamedIndividual .

:eventNumber a owl:DatatypeProperty ;
    rdfs:domain :Event ;
    rdfs:range xsd:int .

:facing a owl:ObjectProperty ;
    rdfs:comment "there is an edge <object1, facing, object2> if object2 is lookable, is visible from object1, and the distance between the centers is < 5 units (~meters). If object1 is a sofa or a chair it should also be turned towards object2" ;
    rdfs:domain x3do:Shape ;
    rdfs:range x3do:Shape ;
    rdfs:subPropertyOf :relatedShape .

:from a owl:ObjectProperty ;
    rdfs:domain :Event ;
    rdfs:range :Room .

:hasActivity a owl:ObjectProperty ;
    rdfs:domain <http://plod.info/rdf/Episode> ;
    rdfs:range ho:Activity .

:has_paper a :Attribute,
        owl:NamedIndividual .

:has_plug a :Attribute,
        owl:NamedIndividual .

:has_surface a :Attribute,
        owl:NamedIndividual .

:has_switch a :Attribute,
        owl:NamedIndividual .

:height a owl:ObjectProperty .

:holds_lh a owl:ObjectProperty ;
    rdfs:comment "analogue of holds_rh for left hand" ;
    rdfs:domain x3do:Shape ;
    rdfs:range x3do:Shape ;
    rdfs:subPropertyOf :relatedShape .

:holds_rh a owl:ObjectProperty ;
    rdfs:comment "edge <character, holds_rh, object> is used to indicate that character holds an object in its right hand" ;
    rdfs:domain x3do:Shape ;
    rdfs:range x3do:Shape ;
    rdfs:subPropertyOf :relatedShape .

:inside a owl:ObjectProperty ;
    rdfs:domain x3do:Shape ;
    rdfs:range x3do:Shape ;
    rdfs:subPropertyOf :relatedShape .

:isStateOf a owl:ObjectProperty ;
    rdfs:domain :State ;
    rdfs:range :Object .

:jumpUp a :Action,
        owl:NamedIndividual .

:kg a :Unit,
        owl:NamedIndividual .

:light a :Attribute,
        owl:NamedIndividual .

:mainObject a owl:ObjectProperty ;
    rdfs:comment """A main object of an event.\r
If an agent pours milk into a glass, the value of the mainObject is the milk.""" ;
    rdfs:domain :Event ;
    rdfs:range :Object ;
    rdfs:subPropertyOf ho:object .

:meter a :Unit,
        owl:NamedIndividual .

:nextActivity a owl:ObjectProperty ;
    rdfs:domain ho:Activity ;
    rdfs:range ho:Activity ;
    rdfs:subPropertyOf :relatedActivity .

:nextEvent a owl:ObjectProperty ;
    rdfs:domain :Event ;
    rdfs:range :Event ;
    rdfs:subPropertyOf :relatedEvent .

:nextSituation a owl:ObjectProperty ;
    rdfs:domain :Situation ;
    rdfs:range :Situation ;
    rdfs:subPropertyOf :relatedSituation ;
    owl:inverseOf :previousSituation .

:nextState a owl:ObjectProperty ;
    rdfs:domain :State ;
    rdfs:range :State ;
    rdfs:subPropertyOf :relatedState ;
    owl:inverseOf :previousState .

:on a owl:ObjectProperty ;
    rdfs:domain x3do:Shape ;
    rdfs:range x3do:Shape ;
    rdfs:subPropertyOf :relatedShape .

:partOf a owl:ObjectProperty ;
    rdfs:domain :State ;
    rdfs:range :Situation .

:place a owl:ObjectProperty ;
    rdfs:domain :Event ;
    rdfs:range :Room .

:previousActivity a owl:ObjectProperty ;
    rdfs:subPropertyOf :relatedActivity .

:previousEvent a owl:ObjectProperty ;
    rdfs:domain :Event ;
    rdfs:range :Event ;
    rdfs:subPropertyOf :relatedEvent .

:recipient a :Attribute,
        owl:NamedIndividual .

:situationAfterEvent a owl:ObjectProperty ;
    rdfs:domain :Event ;
    rdfs:range :Situation ;
    rdfs:subPropertyOf :relatedSituation .

:situationBeforeEvent a owl:ObjectProperty ;
    rdfs:domain :Event ;
    rdfs:range :Situation ;
    rdfs:subPropertyOf :relatedSituation .

:state a owl:ObjectProperty ;
    rdfs:domain :State ;
    rdfs:range :StateType .

:targetObject a owl:ObjectProperty ;
    rdfs:comment """A target object of an event.\r
If an agent pours milk into a glass, the value of the value of the targetObject is the glass.""" ;
    rdfs:domain :Event ;
    rdfs:range :Object ;
    rdfs:subPropertyOf ho:object .

:time a owl:ObjectProperty ;
    rdfs:domain :Event ;
    rdfs:range [ a owl:Class ;
            owl:unionOf ( time:TemporalDuration time:TemporalEntity ) ] ;
    skos:closeMatch <http://purl.org/NET/c4dm/event.owl#time> .

:to a owl:ObjectProperty ;
    rdfs:domain :Event ;
    rdfs:range :Room .

:unit a owl:ObjectProperty ;
    rdfs:range :Unit .

:virtualHome a owl:ObjectProperty ;
    rdfs:range :VirtualHome .

:weight a owl:ObjectProperty .

dcterms:description a owl:AnnotationProperty .

<http://swrl.stanford.edu/ontologies/3.3/swrla.owl#isRuleEnabled> a owl:AnnotationProperty .

ho:Dance a owl:Class ;
    rdfs:comment "The class with sequence of actions for dancing." ;
    rdfs:subClassOf ho:Leisure .

ho:Drink a owl:Class ;
    rdfs:comment """Class that contains sequences where the goal is for the user to drink \r
under different circumstances.""" ;
    rdfs:subClassOf ho:EatingDrinking .

ho:Eat a owl:Class ;
    rdfs:comment """Class with subclasses, for eating seqeunces under different \r
circumstances.""" ;
    rdfs:subClassOf ho:EatingDrinking .

ho:Laugh a owl:Class ;
    rdfs:comment "The class with sequence of actions for laughing." ;
    rdfs:subClassOf ho:Other .

ho:Play a owl:Class ;
    rdfs:comment "The class with sequence of actions on how to play (physical games)." ;
    rdfs:subClassOf ho:Leisure .

ho:Read a owl:Class ;
    rdfs:comment "The class with sequence of actions for  reading." ;
    rdfs:subClassOf ho:Other .

ho:Sew a owl:Class ;
    rdfs:comment "The class with sequence of actions for sewing, from inside the house." ;
    rdfs:subClassOf ho:Other .

ho:Shave a owl:Class ;
    rdfs:comment "The class with sequence of actions for shaving your own face." ;
    rdfs:subClassOf ho:HygieneStyling .

ho:Sit a owl:Class ;
    rdfs:comment "The class with sequence of actions for sitting." ;
    rdfs:subClassOf ho:Other .

ho:Stretch a owl:Class ;
    rdfs:comment "A class with soft physical activity, or exercise, such as stretch." ;
    rdfs:subClassOf ho:PhysicalActivity .

ho:Wait a owl:Class ;
    rdfs:comment "The class with sequence of actions for waiting." ;
    rdfs:subClassOf ho:Other .

ho:Write a owl:Class ;
    rdfs:comment "The class with sequence of actions for writing on a papers or on the computer." ;
    rdfs:subClassOf ho:Other .

ho:add_paper_to_printer a owl:Class ;
    rdfs:comment "The class with sequence of actions for adding paper to the printer." ;
    rdfs:subClassOf ho:Other .

ho:added_meat_to_freezer a owl:Class ;
    rdfs:comment "The class with sequence of actions for adding meat into the freezer." ;
    rdfs:subClassOf ho:HouseArrangement .

ho:admire_art a owl:Class ;
    rdfs:comment """The class with sequence of actions for admiring art that exist inside \r
your home.""" ;
    rdfs:subClassOf ho:Other .

ho:admire_paintings a owl:Class ;
    rdfs:subClassOf ho:Leisure .

ho:annoy_your_dog a owl:Class ;
    rdfs:comment "The class with sequence of actions for annoying your dog, in any room (play with dog)." ;
    rdfs:subClassOf ho:Other .

ho:answer_door a owl:Class ;
    rdfs:comment """The class with sequence of actions for answering the door (main entrance \r
of the house).""" ;
    rdfs:subClassOf ho:SocialInteraction .

ho:answer_emails a owl:Class ;
    rdfs:comment """The class with sequence of actions for answering your mails (writing the \r
text, not sending the mail).""" ;
    rdfs:subClassOf ho:Work .

ho:answer_phone a owl:Class ;
    rdfs:comment "The class with sequence of actions for answering the phone, cell phone or phone home." ;
    rdfs:subClassOf ho:Other .

ho:apply_lotion a owl:Class ;
    rdfs:comment """The class with sequence of actions for applying lotion in any part of \r
the body.""" ;
    rdfs:subClassOf ho:HygieneStyling .

ho:arrange_bookshelf a owl:Class ;
    rdfs:comment "The class with sequence of actions for arranging the bookself." ;
    rdfs:subClassOf ho:HouseArrangement .

ho:arrange_folders a owl:Class ;
    rdfs:comment """The class with sequence of actions for arranging folders, in any place \r
or room.""" ;
    rdfs:subClassOf ho:HouseArrangement .

ho:arrange_furniture a owl:Class ;
    rdfs:comment "The class with sequence of actions for arranging furniture in any room." ;
    rdfs:subClassOf ho:HouseArrangement .

ho:arrange_shoes a owl:Class ;
    rdfs:comment "The class with sequence of actions for arranging shoes in any room." ;
    rdfs:subClassOf ho:HouseArrangement .

ho:arrange_sofa a owl:Class ;
    rdfs:comment "The class with sequence of actions for arranging sofa, in any room." ;
    rdfs:subClassOf ho:HouseArrangement .

ho:bake a owl:Class ;
    rdfs:comment "The class with sequence of actions for baking something." ;
    rdfs:subClassOf ho:FoodPreparation .

ho:bathe a owl:Class ;
    rdfs:comment "The class with sequence of actions for taking a bathe." ;
    rdfs:subClassOf ho:HygieneStyling .

ho:be_able_to_talk_to_me_about_tv_show_im_watching a owl:Class ;
    rdfs:comment """The class with sequence of actions for beeing able to talk to the user \r
about TV show I'm watching.""" ;
    rdfs:subClassOf ho:SocialInteraction .

ho:bed_time a owl:Class ;
    rdfs:comment "The class with sequence of actions for going to bed." ;
    rdfs:subClassOf ho:BedTimeSleep .

ho:blow_dry_hair a owl:Class ;
    rdfs:comment "The class with sequence of actions for blowing and drying your hair." ;
    rdfs:subClassOf ho:HygieneStyling .

ho:break_table a owl:Class ;
    rdfs:comment "The class with sequence of actions for breaking a table, in any room." ;
    rdfs:subClassOf ho:Other .

ho:breakfast a owl:Class ;
    rdfs:comment "The class with sequence of actions for breakfast." ;
    rdfs:subClassOf ho:FoodPreparation .

ho:brew_coffee a owl:Class ;
    rdfs:comment "The class with sequence of actions for brewing coffee in any room." ;
    rdfs:subClassOf ho:FoodPreparation .

ho:bring_dirty_plate_to_sink a owl:Class ;
    rdfs:comment """The class with sequence of actions for bringing your dirty plate in the \r
sink.""" ;
    rdfs:subClassOf ho:HouseArrangement .

ho:bring_food a owl:Class ;
    rdfs:comment "The class with sequence of actions for bringing food, to home from any place." ;
    rdfs:subClassOf ho:Other .

ho:bring_leftovers_in_kitchen a owl:Class ;
    rdfs:comment """The class with sequence of actions for bringing leftovers in kitchen, \r
from any room.""" ;
    rdfs:subClassOf ho:HouseArrangement .

ho:bring_me_red_cookbook a owl:Class ;
    rdfs:comment """The class with sequence of actions for bringing the user the red \r
cookbook.""" ;
    rdfs:subClassOf ho:Other .

ho:broom a owl:Class ;
    rdfs:comment "The class with sequence of actions for broomin, every room in the house." ;
    rdfs:subClassOf ho:HygieneStyling .

ho:browse_computer a owl:Class ;
    rdfs:comment "The class with sequence of actions for browsing the computer." ;
    rdfs:subClassOf ho:Leisure .

ho:browse_internet a owl:Class ;
    rdfs:comment "The class which contains sequences for browsing the internet." ;
    rdfs:subClassOf ho:Leisure,
        ho:Work .

ho:brush_hair a owl:Class ;
    rdfs:comment "The class with sequence of actions for brushing your hair." ;
    rdfs:subClassOf ho:HygieneStyling .

ho:brush_teeth a owl:Class ;
    rdfs:comment "The class with sequence of actions for brushing your teeth." ;
    rdfs:subClassOf ho:HygieneStyling .

ho:build_lego_house a owl:Class ;
    rdfs:comment """The class with sequence of actions for building a lego house, in any \r
room.""" ;
    rdfs:subClassOf ho:Other .

ho:call_client a owl:Class ;
    rdfs:comment """The class with sequence of actions for calling client, either form cell \r
phone or home phone.""" ;
    rdfs:subClassOf ho:SocialInteraction .

ho:call_family_member_with_skype_application a owl:Class ;
    rdfs:comment """The class with sequence of actions for calling family member with skype \r
application.""" ;
    rdfs:subClassOf ho:SocialInteraction .

ho:call_mother a owl:Class ;
    rdfs:comment "The class with sequence of actions for calling your mother." ;
    rdfs:subClassOf ho:SocialInteraction .

ho:card a owl:Class ;
    rdfs:comment "The class with sequence of actions for carding." ;
    rdfs:subClassOf ho:Other .

ho:care_for_houseplants a owl:Class ;
    rdfs:comment "The class with sequence of actions for for carring for house plants." ;
    rdfs:subClassOf ho:HouseArrangement .

ho:carry_box a owl:Class ;
    rdfs:comment "added by virtualhome2kg"@en ;
    rdfs:subClassOf ho:HouseArrangement .

ho:carry_groceries_to_kitchen a owl:Class ;
    rdfs:comment "The class with sequence of actions for carrying groceries to kitchen." ;
    rdfs:subClassOf ho:Other .

ho:celebrate a owl:Class ;
    rdfs:comment "The class with sequence of actions for celebrating, in any occasion." ;
    rdfs:subClassOf ho:Other .

ho:celebrate_birthday_with_nice_meal a owl:Class ;
    rdfs:comment """The class with sequence of actions for celebrating birthday with a nice \r
meal, in any room.""" ;
    rdfs:subClassOf ho:Other .

ho:change_bedding a owl:Class ;
    rdfs:comment """The class with sequence of actions for changing the bedding, in any bed \r
in the house.""" ;
    rdfs:subClassOf ho:HouseArrangement .

ho:change_clothes a owl:Class ;
    rdfs:comment "The class with sequence of actions for changing your own clothes." ;
    rdfs:subClassOf ho:HygieneStyling .

ho:change_curtains a owl:Class ;
    rdfs:comment "The class with sequence of actions for changing curtains, in any room." ;
    rdfs:subClassOf ho:HouseArrangement .

ho:change_light a owl:Class ;
    rdfs:comment "The class with sequence of actions for changing lights in any room." ;
    rdfs:subClassOf ho:HouseArrangement .

ho:change_lightbulb a owl:Class ;
    rdfs:comment "The class with sequence of actions for changing any lightbulb, inside the house." ;
    rdfs:subClassOf ho:HouseArrangement .

ho:change_sheets_and_pillow_cases a owl:Class ;
    rdfs:comment "The class with sequence of actions for changing sheets and pillow cases, for any bed in the house." ;
    rdfs:subClassOf ho:HouseArrangement .

ho:change_sheets_on_bed a owl:Class ;
    rdfs:comment "The class with sequence of actions for changing sheets on bed." ;
    rdfs:subClassOf ho:HouseArrangement .

ho:change_shower_curtain a owl:Class ;
    rdfs:comment "The class with sequence of actions for changing the curtain from a shower." ;
    rdfs:subClassOf ho:HouseArrangement .

ho:change_toilet_paper_roll a owl:Class ;
    rdfs:comment "The class with sequence of actions for changing toilet paper roll." ;
    rdfs:subClassOf ho:HouseArrangement .

ho:change_toothbrush a owl:Class ;
    rdfs:comment """The class with sequence of actions for changing the toothbrush, in any \r
room.""" ;
    rdfs:subClassOf ho:HouseArrangement .

ho:change_tv_channel a owl:Class ;
    rdfs:comment "The class with sequence of actions for changing the tv channel." ;
    rdfs:subClassOf ho:Other .

ho:change_tv_channels a owl:Class ;
    rdfs:comment "The class with sequence of actions for changing TV channels." ;
    rdfs:subClassOf ho:Leisure .

ho:check_appearance_in_mirror a owl:Class ;
    rdfs:comment "The class with sequence of actions for checking appearance in mirror." ;
    rdfs:subClassOf ho:HygieneStyling .

ho:check_email a owl:Class ;
    rdfs:comment """The class with sequence of actions for checking your mail after you have \r
opened it.""" ;
    rdfs:subClassOf ho:Work .

ho:check_homework a owl:Class ;
    rdfs:comment """The class with sequence of actions for checking homework (either you own \r
or anothers person).""" ;
    rdfs:subClassOf ho:Work .

ho:check_self_in_mirror a owl:Class ;
    rdfs:comment "The class with sequence of actions for checking your self in the mirror." ;
    rdfs:subClassOf ho:HygieneStyling .

ho:chop_vegetables a owl:Class ;
    rdfs:comment "Class with sequences on how to cut-chop vegetables in order to prepare dinner, salad, or other kind of food." ;
    rdfs:subClassOf ho:FoodPreparation .

ho:clean a owl:Class ;
    rdfs:comment """Class with general sequences for cleaning, such as clean lamp, bathroom, \r
welcome mat.""" ;
    rdfs:subClassOf ho:HouseCleaning .

ho:clean_bathroom a owl:Class ;
    rdfs:comment """The class with sequence of actions for cleaning the bathroom, the whole \r
room.""" ;
    rdfs:subClassOf ho:HouseCleaning .

ho:clean_desk a owl:Class ;
    rdfs:subClassOf ho:HouseCleaning .

ho:clean_dishes a owl:Class ;
    rdfs:comment "The class with sequence of actions for cleaning the dishes." ;
    rdfs:subClassOf ho:HouseArrangement .

ho:clean_eggs_from_our_chickens a owl:Class ;
    rdfs:comment """The class with sequence of actions for cleaning eggs that were produced \r
by our chickens.""" ;
    rdfs:subClassOf ho:Other .

ho:clean_floor a owl:Class ;
    rdfs:comment "Class with sequences on how to clean the floor." ;
    rdfs:subClassOf ho:HouseCleaning .

ho:clean_fridge a owl:Class ;
    rdfs:comment """The class with sequence of actions clean the fridge form the inside and \r
the outside.""" ;
    rdfs:subClassOf ho:HouseCleaning .

ho:clean_glasses a owl:Class ;
    rdfs:comment "The class with sequence of actions for cleaning watching glasses." ;
    rdfs:subClassOf ho:HouseArrangement .

ho:clean_kitchen a owl:Class ;
    rdfs:comment """The class with sequence of actions the procedure of cleaning all the \r
kitchen.""" ;
    rdfs:subClassOf ho:HouseCleaning .

ho:clean_kitchen_television a owl:Class ;
    rdfs:comment "added by virtualhome2kg"@en ;
    rdfs:subClassOf ho:HouseCleaning .

ho:clean_kitchentable a owl:Class ;
    rdfs:subClassOf ho:HouseCleaning .

ho:clean_large_jacuzzi_tub a owl:Class ;
    rdfs:comment "The class with sequence of actions for cleaning up a large jacuzzi tab." ;
    rdfs:subClassOf ho:HouseCleaning .

ho:clean_living_desk a owl:Class ;
    rdfs:comment "added by virtualhome2kg"@en ;
    rdfs:subClassOf ho:HouseCleaning .

ho:clean_livingroom a owl:Class ;
    rdfs:subClassOf ho:HouseCleaning .

ho:clean_mirror a owl:Class ;
    rdfs:comment """The class with sequence of actions on how to clean a mirror, no matter \r
in which room is in.""" ;
    rdfs:subClassOf ho:HouseCleaning .

ho:clean_room a owl:Class ;
    rdfs:comment "The class with sequence of actions on how to clean a room." ;
    rdfs:subClassOf ho:HouseCleaning .

ho:clean_screen a owl:Class ;
    rdfs:comment "The class with sequence of actions for cleaning the screen of the TV, of a computer, or other objects." ;
    rdfs:subClassOf ho:HouseCleaning .

ho:clean_sink a owl:Class ;
    rdfs:comment """Class with sequences for cleaning only the sink, not the surounding, or \r
the whole room.""" ;
    rdfs:subClassOf ho:HouseCleaning .

ho:clean_slippers a owl:Class ;
    rdfs:subClassOf ho:HouseCleaning .

ho:clean_sofa a owl:Class ;
    rdfs:subClassOf ho:HouseCleaning .

ho:clean_stove a owl:Class ;
    rdfs:comment "added by virtualhome2kg"@en ;
    rdfs:subClassOf ho:HouseCleaning .

ho:clean_television a owl:Class ;
    rdfs:subClassOf ho:HouseCleaning .

ho:clean_toilet a owl:Class ;
    rdfs:comment """Class with sequences on how to clean the toilet specifically, not the \r
whole bathroom.""" ;
    rdfs:subClassOf ho:HouseCleaning .

ho:clear_table a owl:Class ;
    rdfs:comment """The class with sequence of actions for clearing the table after eating \r
or claering it because it is dirty.""" ;
    rdfs:subClassOf ho:HouseArrangement .

ho:close_curtains a owl:Class ;
    rdfs:comment "The class with sequence of actions for clossing the curtains, in any room." ;
    rdfs:subClassOf ho:Other .

ho:close_door a owl:Class ;
    rdfs:comment "The class with sequence of actions for closing the door from any room." ;
    rdfs:subClassOf ho:Other .

ho:close_dresser_drawer a owl:Class ;
    rdfs:comment """The class with sequence of actions for closing dresser drawer, in any \r
room.""" ;
    rdfs:subClassOf ho:Other .

ho:close_shower_curtain a owl:Class ;
    rdfs:comment "The class with sequence of actions for closing shower curtain." ;
    rdfs:subClassOf ho:HouseArrangement .

ho:collect_napkin_rings a owl:Class ;
    rdfs:comment "The class with sequence of actions for collecting napkin rings." ;
    rdfs:subClassOf ho:HouseArrangement .

ho:color a owl:Class ;
    rdfs:comment """The class with sequence of actions for coloring (painting, or painting \r
house, etc.).""" ;
    rdfs:subClassOf ho:Other .

ho:comb_hair a owl:Class ;
    rdfs:comment "The class with sequence of actions for combing cutting your hair." ;
    rdfs:subClassOf ho:HygieneStyling .

ho:come_home a owl:Class ;
    rdfs:comment """The class with sequence of actions for comming home, from wokr, or \r
grocery store, etc.""" ;
    rdfs:subClassOf ho:Other .

ho:come_in_and_leave_home a owl:Class ;
    rdfs:comment """The class with sequence of actions for comming in the house to do \r
something, and then get out again.""" ;
    rdfs:subClassOf ho:Other .

ho:complete_homework a owl:Class ;
    rdfs:comment "The class with sequence of actions for completing your homework." ;
    rdfs:subClassOf ho:Work .

ho:complete_school_work a owl:Class ;
    rdfs:comment """The class with sequence of actions for completing your school work, this \r
is not only homework, could also be getting ready for school.""" ;
    rdfs:subClassOf ho:Work .

ho:complete_surveys_on_amazon_turk a owl:Class ;
    rdfs:comment """The class with sequence of actions for completing youe amazon turk \r
surveys.""" ;
    rdfs:subClassOf ho:Work .

ho:compute a owl:Class ;
    rdfs:comment "The class with sequence of actions for computing anything." ;
    rdfs:subClassOf ho:Other .

ho:computer_work a owl:Class ;
    rdfs:comment "The class with sequence of actions to do computer work." ;
    rdfs:subClassOf ho:Work .

ho:cook_carrot a owl:Class ;
    rdfs:subClassOf ho:FoodPreparation .

ho:cook_food a owl:Class ;
    rdfs:comment "added by virtualhome2kg"@en ;
    rdfs:subClassOf ho:FoodPreparation .

ho:cook_fried_bread a owl:Class ;
    rdfs:subClassOf ho:FoodPreparation .

ho:cook_potato_using_microwave a owl:Class ;
    rdfs:subClassOf ho:FoodPreparation .

ho:cook_potato_using_stove a owl:Class ;
    rdfs:subClassOf ho:FoodPreparation .

ho:cook_salmon a owl:Class ;
    rdfs:subClassOf ho:FoodPreparation .

ho:cook_some_food a owl:Class ;
    rdfs:comment """Class with sequences on how to cook some food prepare the place, the \r
order of the ingredience.""" ;
    rdfs:subClassOf ho:FoodPreparation .

ho:curled_hair a owl:Class ;
    rdfs:comment "The class with sequence of actions for making your hair into curle." ;
    rdfs:subClassOf ho:HygieneStyling .

ho:cut_bread a owl:Class ;
    rdfs:comment "The class with sequence of actions for cutting bread." ;
    rdfs:subClassOf ho:FoodPreparation .

ho:cut_steak a owl:Class ;
    rdfs:comment "The class with sequence of actions for cutting the steak." ;
    rdfs:subClassOf ho:FoodPreparation .

ho:cut_toenails a owl:Class ;
    rdfs:comment "The class with sequence of actions for cutting our toenails." ;
    rdfs:subClassOf ho:HygieneStyling .

ho:cut_your_hair a owl:Class ;
    rdfs:comment "The class with sequence of actions for cutting you hair." ;
    rdfs:subClassOf ho:HygieneStyling .

ho:cutting a owl:Class ;
    rdfs:comment "The class with sequence of actions for cutting any object, in any room." ;
    rdfs:subClassOf ho:Other .

ho:dance_for_table_as_we_eat a owl:Class ;
    rdfs:comment """The class with sequence of actions for dancing for amusement at the \r
table as the persons eat.""" ;
    rdfs:subClassOf ho:EatingDrinking .

ho:dance_with_kids a owl:Class ;
    rdfs:comment "The class with sequence of actions for dancing with kids." ;
    rdfs:subClassOf ho:SocialInteraction .

ho:de-wrinkle_sheet a owl:Class ;
    rdfs:comment "The class with sequence of actions for de-wrinkling sheets." ;
    rdfs:subClassOf ho:HouseCleaning .

ho:de_wrinkle_sheet a owl:Class ;
    rdfs:comment """The class with sequence of actions for de-wrinkling the sheet, in any \r
room.""" ;
    rdfs:subClassOf ho:Other .

ho:decorate a owl:Class ;
    rdfs:comment """The class with sequence of actions for decoratng any item inside the \r
house that can be decorated.""" ;
    rdfs:subClassOf ho:HouseArrangement .

ho:decorate_it a owl:Class ;
    rdfs:comment """The class with sequence of actions for decorating something, after \r
getting the token &quot;decorate it&quot;.""" ;
    rdfs:subClassOf ho:HouseArrangement .

ho:deficate a owl:Class ;
    rdfs:comment "The class with sequence of actions for deficating." ;
    rdfs:subClassOf ho:HygieneStyling .

ho:defrost_chicken a owl:Class ;
    rdfs:comment "The class with sequence of actions for defrosting chicken." ;
    rdfs:subClassOf ho:FoodPreparation .

ho:designing_crafts_with_family a owl:Class ;
    rdfs:comment "The class with sequence of actions for designing crafts with your family." ;
    rdfs:subClassOf ho:Other .

ho:dining a owl:Class ;
    rdfs:comment "The class with sequence of actions for dining." ;
    rdfs:subClassOf ho:EatingDrinking .

ho:do_an_art_project a owl:Class ;
    rdfs:comment """<p style="margin-top: 0">\r
      The class with sequence of actions for doing an art project, in any room.\r
    </p>""" ;
    rdfs:subClassOf ho:Other .

ho:do_dishes a owl:Class ;
    rdfs:comment """The class with sequence of actions for doing the dishes, either clean \r
them or put them in the cabinet""" ;
    rdfs:subClassOf ho:HouseArrangement .

ho:do_facial a owl:Class ;
    rdfs:comment "The class with sequence of actions for doing up a facial." ;
    rdfs:subClassOf ho:HygieneStyling .

ho:do_free-style_dance_routine a owl:Class ;
    rdfs:comment """The class with sequence of actions for doing free style dance routine, \r
in any room.""" ;
    rdfs:subClassOf ho:Other .

ho:do_homework a owl:Class ;
    rdfs:comment """The class with sequence of actions for writing down your homework (or \r
perform other task that will help you finish your homework).""" ;
    rdfs:subClassOf ho:Work .

ho:do_homework_on_paper a owl:Class ;
    rdfs:subClassOf ho:Work .

ho:do_laundry a owl:Class ;
    rdfs:comment "The class with sequence of actions for doing the laundry in any room available." ;
    rdfs:subClassOf ho:HouseArrangement .

ho:do_nails a owl:Class ;
    rdfs:comment "The class with sequence of actions for doing your nails, hands and feet." ;
    rdfs:subClassOf ho:HygieneStyling .

ho:do_research_on_computer a owl:Class ;
    rdfs:subClassOf ho:Work .

ho:do_taxes a owl:Class ;
    rdfs:comment "The class with sequence of actions for doing taxes." ;
    rdfs:subClassOf ho:Work .

ho:do_work a owl:Class ;
    rdfs:comment "The class with sequence of actions for doing work." ;
    rdfs:subClassOf ho:Work .

ho:do_work_on_computer a owl:Class ;
    rdfs:comment """The class with sequence of actions for doing some on the compute, either \r
on iths hardware or on the computer itself.""" ;
    rdfs:subClassOf ho:Work .

ho:do_yoga a owl:Class ;
    rdfs:comment "The class with sequence of actions for doing yoga, in any room." ;
    rdfs:subClassOf ho:PhysicalActivity .

ho:draft_home a owl:Class ;
    rdfs:comment "The class with sequence of actions for drafting a home, in any room." ;
    rdfs:subClassOf ho:Other .

ho:draw_picture a owl:Class ;
    rdfs:comment """The class with sequence of actions for drawing any picture, either on \r
paper or computer.""" ;
    rdfs:subClassOf ho:Other .

ho:dress_up_and_pretend a owl:Class ;
    rdfs:comment """<p style="margin-top: 0">\r
      The class with sequence of actions for dressing up and pretending.\r
    </p>""" ;
    rdfs:subClassOf ho:HygieneStyling .

ho:drink a owl:Class ;
    rdfs:subClassOf ho:EatingDrinking .

ho:drink_alcohol a owl:Class ;
    rdfs:subClassOf ho:EatingDrinking .

ho:drink_alcohol_while_watching_television a owl:Class ;
    rdfs:subClassOf ho:Leisure .

ho:drink_juice a owl:Class ;
    rdfs:subClassOf ho:EatingDrinking .

ho:drink_juice_while_watching_television a owl:Class ;
    rdfs:subClassOf ho:Leisure .

ho:drink_milk a owl:Class ;
    rdfs:subClassOf ho:EatingDrinking .

ho:drink_milk_while_watching_television a owl:Class ;
    rdfs:subClassOf ho:Leisure .

ho:drink_water a owl:Class ;
    rdfs:subClassOf ho:EatingDrinking .

ho:drink_wine a owl:Class ;
    rdfs:subClassOf ho:EatingDrinking .

ho:drink_wine_while_watching_television a owl:Class ;
    rdfs:subClassOf ho:Leisure .

ho:dry_hair a owl:Class ;
    rdfs:comment "The class with sequence of actions for drying your hair." ;
    rdfs:subClassOf ho:HygieneStyling .

ho:dry_soap_bottles a owl:Class ;
    rdfs:comment "The class with sequence of actions for drying soap bottles, in any room." ;
    rdfs:subClassOf ho:Other .

ho:dust a owl:Class ;
    rdfs:comment "Class with sequences about how to dust, different objects." ;
    rdfs:subClassOf ho:HouseCleaning .

ho:eat_bread a owl:Class ;
    rdfs:comment "added by virtualhome2kg"@en ;
    rdfs:subClassOf ho:EatingDrinking .

ho:eat_bread_while_watching_television a owl:Class ;
    rdfs:subClassOf ho:Leisure .

ho:eat_breadslice a owl:Class ;
    rdfs:subClassOf ho:EatingDrinking .

ho:eat_breakfast a owl:Class ;
    rdfs:comment "The class with sequence of actions for eating breakfast in any room." ;
    rdfs:subClassOf ho:FoodPreparation .

ho:eat_breaksfast a owl:Class ;
    rdfs:comment "The class with sequence of actions for eating breakfast only." ;
    rdfs:subClassOf ho:EatingDrinking .

ho:eat_cereal a owl:Class ;
    rdfs:comment "The class with sequence of actions for eating cereals." ;
    rdfs:subClassOf ho:EatingDrinking .

ho:eat_cheese a owl:Class ;
    rdfs:comment "The class with sequence of actions for eating cheese." ;
    rdfs:subClassOf ho:EatingDrinking .

ho:eat_cupcake a owl:Class ;
    rdfs:subClassOf ho:EatingDrinking .

ho:eat_cupcake_while_watching_television a owl:Class ;
    rdfs:subClassOf ho:Leisure .

ho:eat_dessert a owl:Class ;
    rdfs:comment "The class with sequence of actions for eating dessert in any room." ;
    rdfs:subClassOf ho:EatingDrinking .

ho:eat_dinner a owl:Class ;
    rdfs:comment "The class with sequence of actions for eating dinner only." ;
    rdfs:subClassOf ho:EatingDrinking .

ho:eat_donuts a owl:Class ;
    rdfs:comment "The class with sequence of actions for eating donuts." ;
    rdfs:subClassOf ho:EatingDrinking .

ho:eat_family_meals a owl:Class ;
    rdfs:comment "The class with sequence of actions for eating meals with your family." ;
    rdfs:subClassOf ho:EatingDrinking .

ho:eat_ice_cream a owl:Class ;
    rdfs:comment "The class with sequence of actions for eating ice cream in any room." ;
    rdfs:subClassOf ho:EatingDrinking .

ho:eat_meals a owl:Class ;
    rdfs:comment "The class with sequence of actions for eating meals." ;
    rdfs:subClassOf ho:EatingDrinking .

ho:eat_on_fancy_china a owl:Class ;
    rdfs:comment "The class with sequence of actions for eating at fancy china." ;
    rdfs:subClassOf ho:EatingDrinking .

ho:eat_snacks_and_drink_tea a owl:Class ;
    rdfs:comment "The class with sequence of actions for eating snacks and drinking tea." ;
    rdfs:subClassOf ho:EatingDrinking .

ho:eat_while_watching_tv a owl:Class ;
    rdfs:comment """The class with sequence of actions for eating something while watching \r
TV.""" ;
    rdfs:subClassOf ho:EatingDrinking,
        ho:Leisure .

ho:empty_dishwasher_and_fill_dishwasher a owl:Class ;
    rdfs:comment """The class with sequence of actions for emptying dishwasher and fill \r
dishwasher, in any room.""" ;
    rdfs:subClassOf ho:HouseArrangement .

ho:enjoy_view_out_window a owl:Class ;
    rdfs:comment """The class with sequence of actions for enjoying the view out of the \r
window, in any room.""" ;
    rdfs:subClassOf ho:Other .

ho:enter_home a owl:Class ;
    rdfs:comment "The class with sequence of actions for entering home." ;
    rdfs:subClassOf ho:Other .

ho:entertain a owl:Class ;
    rdfs:comment """A class with sequences for entertaining your self with activities that \r
have to do with other persons.""" ;
    rdfs:subClassOf ho:SocialInteraction .

ho:exercise a owl:Class ;
    rdfs:comment "The class with sequence of actions for exercising." ;
    rdfs:subClassOf ho:PhysicalActivity .

ho:face_washing a owl:Class ;
    rdfs:comment "The class with sequence of actions for washing your face." ;
    rdfs:subClassOf ho:HygieneStyling .

ho:fall_backward_while_walking_and_turning a owl:Class ;
    rdfs:subClassOf ho:Abnormal .

ho:fall_in_bathroom a owl:Class ;
    rdfs:subClassOf ho:Abnormal .

ho:fall_sideways_while_walking_forward a owl:Class ;
    rdfs:subClassOf ho:Abnormal .

ho:fall_while_climbing_at_somewhere_height a owl:Class ;
    rdfs:subClassOf ho:Abnormal .

ho:fall_while_during_getting_up_or_rising a owl:Class ;
    rdfs:subClassOf ho:Abnormal .

ho:fall_while_initiation_of_walking a owl:Class ;
    rdfs:subClassOf ho:Abnormal .

ho:fall_while_preparing_meal a owl:Class ;
    rdfs:subClassOf ho:Abnormal .

ho:fall_while_sitting_down a owl:Class ;
    rdfs:subClassOf ho:Abnormal .

ho:fall_while_sitting_down_or_lowering a owl:Class ;
    rdfs:subClassOf ho:Abnormal .

ho:fall_while_standing_and_reaching a owl:Class ;
    rdfs:subClassOf ho:Abnormal .

ho:fall_while_standing_and_turning a owl:Class ;
    rdfs:subClassOf ho:Abnormal .

ho:fall_while_standing_at_somewhere_height a owl:Class ;
    rdfs:subClassOf ho:Abnormal .

ho:fall_while_standing_quietly a owl:Class ;
    rdfs:subClassOf ho:Abnormal .

ho:fall_while_walking_forward a owl:Class ;
    rdfs:subClassOf ho:Abnormal .

ho:family_meetings a owl:Class ;
    rdfs:comment "The class with sequence of actions for family meetings." ;
    rdfs:subClassOf ho:SocialInteraction .

ho:fan_magazines_on_coffee_table a owl:Class ;
    rdfs:comment "The class with sequence of actions for fanning magazines on coffee table." ;
    rdfs:subClassOf ho:Other .

ho:fax_forms_to_doctor a owl:Class ;
    rdfs:comment "The class with sequence of actions to fax forms to a doctor only." ;
    rdfs:subClassOf ho:Work .

ho:feed_daughter a owl:Class ;
    rdfs:comment "The class with sequence of actions for feeding your daughter." ;
    rdfs:subClassOf ho:Other .

ho:feed_dog a owl:Class ;
    rdfs:comment "The class with sequence of actions for feeding the dog." ;
    rdfs:subClassOf ho:Other .

ho:feed_me a owl:Class ;
    rdfs:comment "The class with sequence of actions for feeding the user." ;
    rdfs:subClassOf ho:Other .

ho:file_documents a owl:Class ;
    rdfs:comment "Class with sequences about how to file the documents." ;
    rdfs:subClassOf ho:Work .

ho:file_expense_reports a owl:Class ;
    rdfs:comment "The class with sequence of actions for performing file expense reports." ;
    rdfs:subClassOf ho:Work .

ho:find_dictionary a owl:Class ;
    rdfs:comment "The class with sequence of actions for finding the dictionary, in any room search." ;
    rdfs:subClassOf ho:Other .

ho:find_some_food a owl:Class ;
    rdfs:subClassOf ho:FoodPreparation .

ho:fix_bowl_of_cereal a owl:Class ;
    rdfs:comment """The class with sequence of actions for fixing bowls of cereals (re \r
arrange it if it has spilled, or make it look beautiful).""" ;
    rdfs:subClassOf ho:FoodPreparation .

ho:fix_broken_toys a owl:Class ;
    rdfs:comment """The class with sequence of actions for fixing broken toys, any toys in \r
any room.""" ;
    rdfs:subClassOf ho:Other .

ho:fix_sandwhich a owl:Class ;
    rdfs:comment """The class with sequence of actions for fixing sandwhich (make it look \r
beautifull, or if it has spilled what it has inside re arragne it).""" ;
    rdfs:subClassOf ho:FoodPreparation .

ho:fix_sandwich a owl:Class ;
    rdfs:comment "The class with sequence of actions for fixing a sandwhich." ;
    rdfs:subClassOf ho:FoodPreparation .

ho:fix_snack a owl:Class ;
    rdfs:comment """The class with sequence of actions for fixing a snack (make it look \r
beautiful, or re arrange it if ti has beedn torn apart).""" ;
    rdfs:subClassOf ho:FoodPreparation .

ho:fluff_pillow a owl:Class ;
    rdfs:comment "The class with sequence of actions for fluffing a pillow, in any room." ;
    rdfs:subClassOf ho:HouseArrangement .

ho:fluff_pillows a owl:Class ;
    rdfs:comment "The class with sequence of actions for fluffing the pillows." ;
    rdfs:subClassOf ho:HouseCleaning .

ho:flush_toilet a owl:Class ;
    rdfs:comment "The class with sequence of actions to flush down the toilet." ;
    rdfs:subClassOf ho:HouseCleaning .

ho:fold_clothespants a owl:Class ;
    rdfs:subClassOf ho:HouseArrangement .

ho:fold_clothespile a owl:Class ;
    rdfs:subClassOf ho:HouseArrangement .

ho:fold_clothesshirt a owl:Class ;
    rdfs:subClassOf ho:HouseArrangement .

ho:fold_laundry a owl:Class ;
    rdfs:comment """Class with sequences about how to fold the different laundry objects \r
(i.e. clothes, or objects that could be considered laundry).""" ;
    rdfs:subClassOf ho:HouseArrangement .

ho:gaze_out_window a owl:Class ;
    rdfs:comment "The class with sequence of actions for gazing out the window." ;
    rdfs:subClassOf ho:Other .

ho:get_dressed a owl:Class ;
    rdfs:comment """Class with sequences about how to get dressed for getting out, or for \r
getting to work.""" ;
    rdfs:subClassOf ho:HygieneStyling .

ho:get_drink a owl:Class ;
    rdfs:comment "The class with sequence of actions for getting a drink, in any room." ;
    rdfs:subClassOf ho:Other .

ho:get_glass_of_milk a owl:Class ;
    rdfs:comment """The class with sequence of actions for getting a glass of milk, from any \r
room the milk is in.""" ;
    rdfs:subClassOf ho:Other .

ho:get_glass_of_water a owl:Class ;
    rdfs:comment """The class with sequence of actions for getting glass of water, from any \r
room that can get water.""" ;
    rdfs:subClassOf ho:Other .

ho:get_in_way_of_guests_trying_to_leave a owl:Class ;
    rdfs:comment "The class with sequence of actions for getting in way of guests." ;
    rdfs:subClassOf ho:Other .

ho:get_mail_ready a owl:Class ;
    rdfs:comment "The class with sequence of actions for getting an email ready to be send." ;
    rdfs:subClassOf ho:Work .

ho:get_out_dish a owl:Class ;
    rdfs:comment """The class with sequence of actions for getting a dish out, for serving \r
in any room.""" ;
    rdfs:subClassOf ho:Other .

ho:get_out_of_bed a owl:Class ;
    rdfs:subClassOf ho:BedTimeSleep .

ho:get_ready_for_bed a owl:Class ;
    rdfs:comment "\\The class with sequence of actions for getting ready for going to bed." ;
    rdfs:subClassOf ho:BedTimeSleep .

ho:get_ready_for_day a owl:Class ;
    rdfs:comment "The class with sequence of actions for getting ready for the day." ;
    rdfs:subClassOf ho:GettingReady .

ho:get_ready_for_school a owl:Class ;
    rdfs:comment "The class with sequence of actions for getting ready for school." ;
    rdfs:subClassOf ho:GettingReady .

ho:get_ready_for_work a owl:Class ;
    rdfs:comment "The class with sequence of actions for gettinf ready to go to work." ;
    rdfs:subClassOf ho:GettingReady .

ho:get_ready_to_leave a owl:Class ;
    rdfs:comment "The class with sequence of actions for getting ready to leave the house." ;
    rdfs:subClassOf ho:GettingReady .

ho:get_some_water a owl:Class ;
    rdfs:comment "The class with sequence of actions for getting some water." ;
    rdfs:subClassOf ho:Other .

ho:get_something_to_drink a owl:Class ;
    rdfs:comment "The class with sequence of actions for getting something to drink." ;
    rdfs:subClassOf ho:EatingDrinking .

ho:get_toilet_paper a owl:Class ;
    rdfs:comment """The class with sequence of actions for getting toilet paper from any \r
room and put it in the toilet.""" ;
    rdfs:subClassOf ho:Other .

ho:getting__dresses a owl:Class ;
    rdfs:comment "The class with sequence of actions for getting dresses." ;
    rdfs:subClassOf ho:Other .

ho:getting_dressed a owl:Class ;
    rdfs:comment "The class with sequence of actions for getting dressed." ;
    rdfs:subClassOf ho:HygieneStyling .

ho:getting_in_way_of_guest_trying_to_leave a owl:Class ;
    rdfs:comment """The class with sequence of actions for getting in way of guest trying to \r
leave.""" ;
    rdfs:subClassOf ho:SocialInteraction .

ho:give_children_bath a owl:Class ;
    rdfs:comment "The class with sequence of actions for giving the children a bath.",
        "The class with sequence of actions for giving your children a bath." ;
    rdfs:subClassOf ho:HygieneStyling,
        ho:SocialInteraction .

ho:give_me_bath a owl:Class ;
    rdfs:comment "The class with sequence of actions for giving a bath to the user." ;
    rdfs:subClassOf ho:HygieneStyling .

ho:give_milk_to_cat a owl:Class ;
    rdfs:comment """The class with sequence of actions for giving milk to the cat, inside \r
the house, but in any room.""" ;
    rdfs:subClassOf ho:Other .

ho:give_your_child_bath a owl:Class ;
    rdfs:comment "The class with sequence of actions for giving you child bath." ;
    rdfs:subClassOf ho:HygieneStyling .

ho:go_pee a owl:Class ;
    rdfs:comment "The class with sequence of actions for going to pee." ;
    rdfs:subClassOf ho:HygieneStyling .

ho:go_to_bathroom a owl:Class ;
    rdfs:comment "The class with sequence of actions for going to the bathroom." ;
    rdfs:subClassOf ho:HygieneStyling .

ho:go_to_bed a owl:Class ;
    rdfs:comment "The class with sequence of actions for going to bed." ;
    rdfs:subClassOf ho:BedTimeSleep .

ho:go_to_sleep a owl:Class ;
    rdfs:comment """A class with sequences on how to go to sleep, or get ready to go to \r
sleep.""" ;
    rdfs:subClassOf ho:BedTimeSleep .

ho:go_to_toilet a owl:Class ;
    rdfs:comment "Class with seqeunces on how to go to toilet." ;
    rdfs:subClassOf ho:HygieneStyling .

ho:grab_some_juice a owl:Class ;
    rdfs:comment """The class with sequence of actions for grabing some juice, from the \r
fridge or elsewhere.""" ;
    rdfs:subClassOf ho:Other .

ho:grab_things a owl:Class ;
    rdfs:comment "The class with sequence of actions for grabing things, any object." ;
    rdfs:subClassOf ho:Other .

ho:grading_papers a owl:Class ;
    rdfs:comment """The class with sequence of actions for grading some papers (usually for \r
school).""" ;
    rdfs:subClassOf ho:Work .

ho:greet_guests a owl:Class ;
    rdfs:comment "A class with sequences for greeting guest that have come to your home for visit" ;
    rdfs:subClassOf ho:SocialInteraction .

ho:greet_people a owl:Class ;
    rdfs:comment "The class with sequence of actions for greeting people in any room or outside the house." ;
    rdfs:subClassOf ho:SocialInteraction .

ho:hair a owl:Class ;
    rdfs:comment "The class with sequence of actions for hairing." ;
    rdfs:subClassOf ho:Other .

ho:hair_dressing a owl:Class ;
    rdfs:comment "The class with sequence of actions for hair dressing." ;
    rdfs:subClassOf ho:HygieneStyling .

ho:hand_washing a owl:Class ;
    rdfs:comment "The class with sequence of actions for hand washing, in any room." ;
    rdfs:subClassOf ho:HygieneStyling .

ho:hang_car_keys a owl:Class ;
    rdfs:comment """The class with sequence of actions for hanging car keys, in any place \r
that can be hanged.""" ;
    rdfs:subClassOf ho:Other .

ho:hang_keys a owl:Class ;
    rdfs:comment "The class with sequence of actions for hanging up keys in any room." ;
    rdfs:subClassOf ho:Other .

ho:hang_out a owl:Class ;
    rdfs:comment "The class with sequence of actions for hanging out, speending free time in house." ;
    rdfs:subClassOf ho:Other .

ho:hang_pictures a owl:Class ;
    rdfs:comment "The class with sequence of actions for hanging out a picture in any room." ;
    rdfs:subClassOf ho:HouseArrangement .

ho:hang_up_car_keys a owl:Class ;
    rdfs:comment """The class with sequence of actions for hanging up your car keys, in \r
every room.""" ;
    rdfs:subClassOf ho:Other .

ho:hang_up_jacket a owl:Class ;
    rdfs:comment """A class with sequences on how to hang up your jacket\r
.""" ;
    rdfs:subClassOf ho:Other .

ho:hang_up_poster a owl:Class ;
    rdfs:comment "The class with sequence of actions for hanging up the poster in any room." ;
    rdfs:subClassOf ho:HouseArrangement .

ho:hang_with_friend a owl:Class ;
    rdfs:comment """The class with sequence of actions for hanging with your friend inside \r
the house.""" ;
    rdfs:subClassOf ho:SocialInteraction .

ho:hang_with_friends a owl:Class ;
    rdfs:comment "The class with sequence of actions for hanging with friends." ;
    rdfs:subClassOf ho:Other .

ho:have_conversation_with_boyfriend a owl:Class ;
    rdfs:comment """The class with sequence of actions for having conversation with your \r
boyfriend.""" ;
    rdfs:subClassOf ho:SocialInteraction .

ho:have_dinner a owl:Class ;
    rdfs:comment "The class with sequence of actions for having dinner." ;
    rdfs:subClassOf ho:EatingDrinking .

ho:have_evening_beverage a owl:Class ;
    rdfs:subClassOf ho:EatingDrinking .

ho:have_ice_coffee a owl:Class ;
    rdfs:comment "The class with sequence of actions for drinking ice coffee in any room." ;
    rdfs:subClassOf ho:EatingDrinking .

ho:have_morning_beverage a owl:Class ;
    rdfs:subClassOf ho:EatingDrinking .

ho:have_party a owl:Class ;
    rdfs:comment "The class with sequence of actions for having a party inside the house." ;
    rdfs:subClassOf ho:SocialInteraction .

ho:have_quality_family_time a owl:Class ;
    rdfs:comment "The class with sequence of actions for having qualtiy family time, no matter the members if the family." ;
    rdfs:subClassOf ho:SocialInteraction .

ho:have_snack a owl:Class ;
    rdfs:comment """The class with sequence of actions for having a snack at any time of the \r
day.""" ;
    rdfs:subClassOf ho:EatingDrinking .

ho:have_tea_party a owl:Class ;
    rdfs:comment "The class with sequence of actions for having a tea party." ;
    rdfs:subClassOf ho:SocialInteraction .

ho:help_kids_with_homework a owl:Class ;
    rdfs:comment "The class with sequence of actions for helping kids with their homework." ;
    rdfs:subClassOf ho:SocialInteraction .

ho:help_organize_files a owl:Class ;
    rdfs:comment """The class with sequence of actions for helping organize the files, in \r
any order.""" ;
    rdfs:subClassOf ho:Other .

ho:help_with_quiz_shows a owl:Class ;
    rdfs:comment """The class with sequence of actions for helping with quiz shows, any \r
person.""" ;
    rdfs:subClassOf ho:Other .

ho:hide a owl:Class ;
    rdfs:comment "The class with sequence of actions for hiding in any room." ;
    rdfs:subClassOf ho:Other .

ho:hold_coats_and_umbrellas a owl:Class ;
    rdfs:comment """The class with sequence of actions for holding your coat (or coats) and \r
an umbrella.""" ;
    rdfs:subClassOf ho:HouseArrangement .

ho:homework a owl:Class ;
    rdfs:comment "The class with sequence of actions for actions for getting ready for homework." ;
    rdfs:subClassOf ho:Work .

ho:ignore_people a owl:Class ;
    rdfs:comment "The class with sequence of actions for ignoring the people inside the room." ;
    rdfs:subClassOf ho:SocialInteraction .

ho:in_living_room_i_eat_dinner a owl:Class ;
    rdfs:comment "The class with sequence of actions for eating dinner in living room." ;
    rdfs:subClassOf ho:Leisure .

ho:iron_shirt a owl:Class ;
    rdfs:comment """The class with sequence of actions for ironing a shirt in any place or \r
room.""" ;
    rdfs:subClassOf ho:HouseArrangement .

ho:juggling a owl:Class ;
    rdfs:comment """The class with sequence of actions for juggling (whatever object can \r
fly).""" ;
    rdfs:subClassOf ho:Leisure .

ho:keep_an_eye_on_stove_as_something_is_cooking a owl:Class ;
    rdfs:comment """The class with sequence of actions for keeping an eye on stove as \r
somehting is cooking.""" ;
    rdfs:subClassOf ho:FoodPreparation .

ho:keep_cats_inside_while_door_is_open a owl:Class ;
    rdfs:comment """The class with sequence of actions for trying to keep cats inside while \r
door is open.""" ;
    rdfs:subClassOf ho:Other .

ho:keep_cats_out_of_room a owl:Class ;
    rdfs:comment """The class with sequence of actions for keepin the cats out of room\r
, any room.""" ;
    rdfs:subClassOf ho:SocialInteraction .

ho:lay_down_on_floor_and_say_im_rug a owl:Class ;
    rdfs:comment """The class with sequence of actions for laying down on floor in any room \r
and say, I am rug.""" ;
    rdfs:subClassOf ho:Other .

ho:lay_tablecloth a owl:Class ;
    rdfs:comment """The class with sequence of actions for laying the tablecoth on the \r
table, in any room.""" ;
    rdfs:subClassOf ho:HouseArrangement .

ho:leave_home a owl:Class ;
    rdfs:comment "The class with sequence of actions for leaving home." ;
    rdfs:subClassOf ho:Other .

ho:leaving_room a owl:Class ;
    rdfs:comment "added by virtualhome2kg"@en ;
    rdfs:subClassOf ho:Other .

ho:legopp a owl:Class ;
    rdfs:subClassOf ho:PhysicalActivity .

ho:let_baby_learn_how_to_walk a owl:Class ;
    rdfs:comment "The class with sequence of actions for letting the baby learn how to walk." ;
    rdfs:subClassOf ho:Other .

ho:let_bay_learn_how_to_walk a owl:Class ;
    rdfs:comment """The class with sequence of actions for letting your child or baby to \r
learn how to walk.""" ;
    rdfs:subClassOf ho:SocialInteraction .

ho:light_candle a owl:Class ;
    rdfs:comment "The class with sequence of actions for lighting up a candle in any room." ;
    rdfs:subClassOf ho:Other .

ho:light_candles a owl:Class ;
    rdfs:comment "The class with sequence of actions for lighting up the candles." ;
    rdfs:subClassOf ho:HouseArrangement .

ho:listen_to_music a owl:Class ;
    rdfs:comment "The class which contains sequences for listening to music." ;
    rdfs:subClassOf ho:Leisure .

ho:load_dishwasher a owl:Class ;
    rdfs:comment """The class with sequence of actions for laoding up the dishwasher\r
.""" ;
    rdfs:subClassOf ho:HouseArrangement .

ho:lock_door a owl:Class ;
    rdfs:comment "The class with sequence of actions for locking the door in any room." ;
    rdfs:subClassOf ho:Other .

ho:look_at_mirror a owl:Class ;
    rdfs:comment "The class with sequence of actions for looking at the mirror in any room." ;
    rdfs:subClassOf ho:Other .

ho:look_at_painting a owl:Class ;
    rdfs:comment "The class with sequence of actions for looki g at painting in any room." ;
    rdfs:subClassOf ho:Other .

ho:look_in_refrigerator a owl:Class ;
    rdfs:comment """The class with sequence of actions for looking in refrigerator for any \r
reason.""" ;
    rdfs:subClassOf ho:Other .

ho:look_out_window a owl:Class ;
    rdfs:comment """The class with sequence of actions for looking out the window, in any \r
room.""" ;
    rdfs:subClassOf ho:Other .

ho:mail_signed_letter_to_customer a owl:Class ;
    rdfs:comment """The class with sequence of actions read-send a mail that contains a \r
signed letter for the customer.""" ;
    rdfs:subClassOf ho:Work .

ho:make__cookies a owl:Class ;
    rdfs:comment "The class with sequence of actions for making cookies in any room." ;
    rdfs:subClassOf ho:FoodPreparation .

ho:make_banana_bread a owl:Class ;
    rdfs:comment """The class with sequence of actions for making a bread that contains \r
banana.""" ;
    rdfs:subClassOf ho:FoodPreparation .

ho:make_bed a owl:Class ;
    rdfs:comment """Class with sequences about how to make you own bed, under different \r
circumstances.""" ;
    rdfs:subClassOf ho:HouseArrangement .

ho:make_cereal a owl:Class ;
    rdfs:comment "The class with sequence of actions for making cereals." ;
    rdfs:subClassOf ho:FoodPreparation .

ho:make_childs_bed a owl:Class ;
    rdfs:comment "The class with sequence of actions for making the childs bed in any room." ;
    rdfs:subClassOf ho:HouseArrangement .

ho:make_coffee a owl:Class ;
    rdfs:comment "Class with sequences on how to make coffee with different methods, and different steps." ;
    rdfs:subClassOf ho:FoodPreparation .

ho:make_cold_cereal a owl:Class ;
    rdfs:subClassOf ho:FoodPreparation .

ho:make_drink a owl:Class ;
    rdfs:comment "The class with sequence of actions for making a drink." ;
    rdfs:subClassOf ho:FoodPreparation .

ho:make_eggs a owl:Class ;
    rdfs:comment "The class with sequence of actions for making eggs." ;
    rdfs:subClassOf ho:FoodPreparation .

ho:make_hot_cereal a owl:Class ;
    rdfs:subClassOf ho:FoodPreparation .

ho:make_ice_in_ice_trays_for_freezer a owl:Class ;
    rdfs:comment """The class with sequence of actions for making ice in ice trays fo \r
freezer.""" ;
    rdfs:subClassOf ho:FoodPreparation .

ho:make_iced_coffee a owl:Class ;
    rdfs:comment "The class with sequence of actions for making iced coffee only." ;
    rdfs:subClassOf ho:FoodPreparation .

ho:make_jello a owl:Class ;
    rdfs:comment "The class with sequence of actions for making jello." ;
    rdfs:subClassOf ho:FoodPreparation .

ho:make_kids_bed a owl:Class ;
    rdfs:comment "The class with sequence of actions for making the kids bed, in any room." ;
    rdfs:subClassOf ho:HouseArrangement .

ho:make_peanut_butter_sandwhich a owl:Class ;
    rdfs:comment "The class with sequence of actions for making peanut butter sandwhich." ;
    rdfs:subClassOf ho:FoodPreparation .

ho:make_peanut_butter_sandwich a owl:Class ;
    rdfs:comment "The class with sequence of actions for making peanut butter sandwhich." ;
    rdfs:subClassOf ho:FoodPreparation .

ho:make_phone_call a owl:Class ;
    rdfs:comment "The class with sequence of actions for making a phone call, form cell phone or home phone." ;
    rdfs:subClassOf ho:SocialInteraction .

ho:make_place_cards a owl:Class ;
    rdfs:comment "The class with sequence of actions for making place cards." ;
    rdfs:subClassOf ho:Other .

ho:make_popcorn a owl:Class ;
    rdfs:comment """The class with sequence of actions for making popcorn, in what ever mean \r
can cook popcorn.""" ;
    rdfs:subClassOf ho:FoodPreparation .

ho:make_sandwich a owl:Class ;
    rdfs:comment "The class with sequence of actions for making sandwich." ;
    rdfs:subClassOf ho:FoodPreparation .

ho:make_sandwitch a owl:Class ;
    rdfs:comment "The class with sequence of actions for making a sandwitch." ;
    rdfs:subClassOf ho:FoodPreparation .

ho:make_several_copies_on_printer a owl:Class ;
    rdfs:comment """The class with sequence of actions to make several copies on the \r
printer, the file does not matter in this case.""" ;
    rdfs:subClassOf ho:Work .

ho:make_tea a owl:Class ;
    rdfs:comment "The class with sequence of actions for making tea." ;
    rdfs:subClassOf ho:FoodPreparation .

ho:make_toast a owl:Class ;
    rdfs:comment """The class with sequence of actions for making your own toast, or for \r
someone else.""" ;
    rdfs:subClassOf ho:FoodPreparation .

ho:make_tomato_sauce a owl:Class ;
    rdfs:comment """The class with sequence of actions for making tomatoes sauce, in any \r
room.""" ;
    rdfs:subClassOf ho:FoodPreparation .

ho:make_tutu a owl:Class ;
    rdfs:comment "The class with sequence of actions for making tutu, inside the house." ;
    rdfs:subClassOf ho:Other .

ho:make_up_bed_for_guest_on_couch a owl:Class ;
    rdfs:comment """The class with sequence of actions for making up bed for guest on couch, \r
wherever the couch is in the house.""" ;
    rdfs:subClassOf ho:HouseArrangement .

ho:manage_documents a owl:Class ;
    rdfs:comment "The class with sequence of actions on how to manage your documents." ;
    rdfs:subClassOf ho:Work .

ho:manage_emails a owl:Class ;
    rdfs:comment """The class with sequence of actions for managing your emails (sorting, or \r
merging the different files with emails).""" ;
    rdfs:subClassOf ho:Work .

ho:massage a owl:Class ;
    rdfs:comment "The class with sequence of actions for doing massage in any room." ;
    rdfs:subClassOf ho:SocialInteraction .

ho:meeting a owl:Class ;
    rdfs:comment """The class with sequence of actions for meeting , no matter the purpose \r
of meeting.""" ;
    rdfs:subClassOf ho:SocialInteraction .

ho:mop a owl:Class ;
    rdfs:comment "The class with sequence of actions taking up the mop and cleaning." ;
    rdfs:subClassOf ho:HouseCleaning .

ho:mop_floor a owl:Class ;
    rdfs:comment "The class with sequence of actions for mopping the floor." ;
    rdfs:subClassOf ho:HouseCleaning .

ho:movie a owl:Class ;
    rdfs:comment """The class with sequence of actions for watching a movie, either at TV or \r
your Laptop.""" ;
    rdfs:subClassOf ho:Leisure .

ho:oil_dining_room a owl:Class ;
    rdfs:comment "The class with sequence of actions for oiling dining room." ;
    rdfs:subClassOf ho:HouseCleaning .

ho:open_bathroom_window a owl:Class ;
    rdfs:comment "The class with sequence of actions for opening bathroom window." ;
    rdfs:subClassOf ho:Other .

ho:open_curtains a owl:Class ;
    rdfs:comment """The class with sequence of actions for opening up the curtains, from any \r
room inside the house.""" ;
    rdfs:subClassOf ho:Other .

ho:open_door a owl:Class ;
    rdfs:comment """The class with sequence of actions for opening the door, either from the \r
main entrance or door of a room.""" ;
    rdfs:subClassOf ho:Other .

ho:open_door_and_great_guests a owl:Class ;
    rdfs:comment "The class with sequence of actions for opening the door and greeting guests." ;
    rdfs:subClassOf ho:SocialInteraction .

ho:open_front_door a owl:Class ;
    rdfs:comment """The class with sequence of actions for opening front door (main entrance \r
door).""" ;
    rdfs:subClassOf ho:Other .

ho:open_window a owl:Class ;
    rdfs:comment "The class with sequence of actions for opening a window in any room." ;
    rdfs:subClassOf ho:Other .

ho:order_office_suplies a owl:Class ;
    rdfs:comment """The class with sequence of actions for ordering office suplies, such as \r
papers, writing material, and more.""" ;
    rdfs:subClassOf ho:Work .

ho:organise_paperwork a owl:Class ;
    rdfs:comment "The class with sequence of actions for organizing paperwork." ;
    rdfs:subClassOf ho:Work .

ho:organize a owl:Class ;
    rdfs:comment """The class with sequence of actions for organizing your work, your \r
clothes, etc.""" ;
    rdfs:subClassOf ho:Other .

ho:organize_cabinet a owl:Class ;
    rdfs:comment """The class with sequence of actions for organizing the objects insde the \r
cabinet.""" ;
    rdfs:subClassOf ho:HouseArrangement .

ho:organize_closet a owl:Class ;
    rdfs:comment "The class with sequence of actions for organizing the closet." ;
    rdfs:subClassOf ho:HouseArrangement,
        ho:HouseCleaning .

ho:organize_desk a owl:Class ;
    rdfs:comment """The class with sequence of actions for organizing the desk place, \r
sorting items, pick up items.""" ;
    rdfs:subClassOf ho:HouseArrangement .

ho:organize_files a owl:Class ;
    rdfs:comment "The class with sequence of actions for organizing files, in anu order desired." ;
    rdfs:subClassOf ho:Other .

ho:organize_panrty a owl:Class ;
    rdfs:comment """The class with sequence of actions for organizing party, by using your \r
phone or computer.""" ;
    rdfs:subClassOf ho:HouseArrangement .

ho:organize_paperwork a owl:Class ;
    rdfs:comment "The class with sequence of actions for organizing your paper work." ;
    rdfs:subClassOf ho:Work .

ho:pack_lunch a owl:Class ;
    rdfs:comment "The class with sequence of actions for packing up lunch, and go anywhere." ;
    rdfs:subClassOf ho:Other .

ho:paint_ceiling a owl:Class ;
    rdfs:comment "The class with sequence of actions for painting the ceiling only." ;
    rdfs:subClassOf ho:HouseArrangement .

ho:paint_nails a owl:Class ;
    rdfs:comment "The class with sequence of actions for painting your own nails." ;
    rdfs:subClassOf ho:HygieneStyling .

ho:pay_bills a owl:Class ;
    rdfs:comment "Class that contains sequences about how to pay bills." ;
    rdfs:subClassOf ho:Work .

ho:pee a owl:Class ;
    rdfs:comment "The class with sequence of actions for peeing." ;
    rdfs:subClassOf ho:HygieneStyling .

ho:peel_kiwi a owl:Class ;
    rdfs:comment "The class with sequence of actions for pelling the kiwi fruit." ;
    rdfs:subClassOf ho:FoodPreparation .

ho:peel_potatoes a owl:Class ;
    rdfs:comment "The class with sequence of actions for peeling potatoes in any room." ;
    rdfs:subClassOf ho:FoodPreparation .

ho:pet_cat a owl:Class ;
    rdfs:comment "A class with sequeces on how to pet your cat.." ;
    rdfs:subClassOf ho:SocialInteraction .

ho:pet_dog a owl:Class ;
    rdfs:comment "The class with sequence of actions for petting your dog." ;
    rdfs:subClassOf ho:Other .

ho:physical_therapy a owl:Class ;
    rdfs:comment "The class with sequence of actions for doing physical therapy." ;
    rdfs:subClassOf ho:PhysicalActivity .

ho:pick_toys a owl:Class ;
    rdfs:comment """The class with sequence of actions for picking up toys that were thrown \r
away.""" ;
    rdfs:subClassOf ho:HouseArrangement .

ho:pick_up a owl:Class ;
    rdfs:comment """The class with sequence of actions for picking up any object, in any \r
room.""" ;
    rdfs:subClassOf ho:Other .

ho:pick_up_all_trash a owl:Class ;
    rdfs:comment """The class with sequence of actions for picking up all trash from the \r
floor, or any other place.""" ;
    rdfs:subClassOf ho:Other .

ho:pick_up_cat_hair a owl:Class ;
    rdfs:comment "The class with sequence of actions picking up the cat hair from the various furniture and the floor." ;
    rdfs:subClassOf ho:HouseCleaning .

ho:pick_up_dIshes a owl:Class ;
    rdfs:comment "The class with sequence of actions for picking up the dishes, from any room." ;
    rdfs:subClassOf ho:HouseArrangement .

ho:pick_up_dirty_dishes a owl:Class ;
    rdfs:comment """The class with sequence of actions for picking up dirty dishes, in any \r
room.""" ;
    rdfs:subClassOf ho:HouseArrangement .

ho:pick_up_dirty_fork a owl:Class ;
    rdfs:subClassOf ho:HouseArrangement .

ho:pick_up_dirty_knife a owl:Class ;
    rdfs:subClassOf ho:HouseArrangement .

ho:pick_up_dirty_waterglass a owl:Class ;
    rdfs:subClassOf ho:HouseArrangement .

ho:pick_up_dirty_wineglass a owl:Class ;
    rdfs:subClassOf ho:HouseArrangement .

ho:pick_up_dishes a owl:Class ;
    rdfs:comment "The class with sequence of actions for picking up the dishes." ;
    rdfs:subClassOf ho:Other .

ho:pick_up_obvious_trash a owl:Class ;
    rdfs:comment """The class with sequence of actions for picking up objects that are \r
obiously trash.""" ;
    rdfs:subClassOf ho:Other .

ho:pick_up_phone a owl:Class ;
    rdfs:comment """A class with sequences on how to answer the phone, from different rooms, \r
and in different scenaria sucks as holding something in hands, etc.""" ;
    rdfs:subClassOf ho:Other .

ho:pick_up_spare_change_on_dresser a owl:Class ;
    rdfs:comment "The class with sequence of actions for picking up sparse change on dresser, in any room." ;
    rdfs:subClassOf ho:Other .

ho:pick_up_toys a owl:Class ;
    rdfs:comment """A class with sequences on to pick up the toys left behind by other \r
individuals.""" ;
    rdfs:subClassOf ho:Other .

ho:place_bathmat a owl:Class ;
    rdfs:comment "The class with sequence of actions for placing bathmat in the bathroom." ;
    rdfs:subClassOf ho:HouseArrangement .

ho:place_centerpiece a owl:Class ;
    rdfs:comment "The class with sequence of actions for placing centerpiece." ;
    rdfs:subClassOf ho:HouseArrangement .

ho:place_fork a owl:Class ;
    rdfs:subClassOf ho:HouseArrangement .

ho:place_knife a owl:Class ;
    rdfs:subClassOf ho:HouseArrangement .

ho:place_plate a owl:Class ;
    rdfs:subClassOf ho:HouseArrangement .

ho:place_table a owl:Class ;
    rdfs:comment "The class with sequence of actions for placing the table in any room." ;
    rdfs:subClassOf ho:HouseArrangement .

ho:place_waterglass a owl:Class ;
    rdfs:subClassOf ho:HouseArrangement .

ho:place_wine a owl:Class ;
    rdfs:subClassOf ho:HouseArrangement .

ho:place_wineglass a owl:Class ;
    rdfs:subClassOf ho:HouseArrangement .

ho:play_fetch_with_dog a owl:Class ;
    rdfs:comment "The class with sequence of actions for playing fetch with a dog." ;
    rdfs:subClassOf ho:SocialInteraction .

ho:play_games a owl:Class ;
    rdfs:comment "The sequence of actions about how to paly games." ;
    rdfs:subClassOf ho:Leisure .

ho:play_guitar a owl:Class ;
    rdfs:comment """The class with sequence of actions for playing with the guitar (electric \r
or normal).""" ;
    rdfs:subClassOf ho:Leisure .

ho:play_musical_chairs a owl:Class ;
    rdfs:comment "The class with sequence of actions for playing musical chairs, (with no respect to the environment)." ;
    rdfs:subClassOf ho:Leisure .

ho:play_on_laptop a owl:Class ;
    rdfs:comment "The class with sequence of actions for palying games or have fyn while at your computer." ;
    rdfs:subClassOf ho:Leisure .

ho:play_piano a owl:Class ;
    rdfs:comment "The class with sequence of actions for playing your piano." ;
    rdfs:subClassOf ho:Leisure .

ho:play_with_barbies a owl:Class ;
    rdfs:comment """<p style="margin-top: 0">\r
      The class with sequence of actions for palying with barbie dolls.\r
    </p>""" ;
    rdfs:subClassOf ho:Leisure .

ho:play_with_toys a owl:Class ;
    rdfs:comment "The class with sequence of actions for playing with toys, in any room." ;
    rdfs:subClassOf ho:Other .

ho:playing_video_game a owl:Class ;
    rdfs:comment """The class with sequence of actions either at a console or at the \r
computer.""" ;
    rdfs:subClassOf ho:Leisure .

ho:playtime_lunch_with_dolls a owl:Class ;
    rdfs:comment """The class with sequence of actions for playing with dolls while eating \r
your lunch.""" ;
    rdfs:subClassOf ho:Leisure .

ho:plug_in_nightlight a owl:Class ;
    rdfs:comment "The class with sequence of actions for pluging in the nightlight, in any room." ;
    rdfs:subClassOf ho:Other .

ho:polish_table a owl:Class ;
    rdfs:comment "The class with sequence of actions to polish a table." ;
    rdfs:subClassOf ho:HouseCleaning .

ho:polish_teas_pot a owl:Class ;
    rdfs:comment """The class with sequence of actions for polishing tea pots\r
.""" ;
    rdfs:subClassOf ho:HouseArrangement .

ho:polish_your_shoes a owl:Class ;
    rdfs:comment "The class with sequence of actions for polishing your own shoes." ;
    rdfs:subClassOf ho:HouseArrangement .

ho:polishing_floor a owl:Class ;
    rdfs:comment "The class with sequence of actions for polishing the floor." ;
    rdfs:subClassOf ho:HouseCleaning .

ho:pop_zit a owl:Class ;
    rdfs:comment "The class with sequence of actions for poping out zits." ;
    rdfs:subClassOf ho:Other .

ho:pour_cup_of_coffee a owl:Class ;
    rdfs:comment "The class with sequence of actions for pouring cup of coffee." ;
    rdfs:subClassOf ho:Other .

ho:practice_own_singing a owl:Class ;
    rdfs:comment "The class with sequence of actions for practicing your own singing." ;
    rdfs:subClassOf ho:Leisure .

ho:practice_violin a owl:Class ;
    rdfs:comment "The class with sequence of actions for practicing your violin." ;
    rdfs:subClassOf ho:Leisure .

ho:praying a owl:Class ;
    rdfs:comment "The class with sequence of actions for praying in any room." ;
    rdfs:subClassOf ho:Other .

ho:prepare_breakfast a owl:Class ;
    rdfs:comment """The class with sequence of actions for preparing the breakfast (not \r
eating the breakfast).""" ;
    rdfs:subClassOf ho:FoodPreparation .

ho:prepare_dinner a owl:Class ;
    rdfs:comment "Class with sequences for the procedure of getting the able ready to eat dinner.",
        "The class with sequence of actions for making the dinner (the procedure of cooking)." ;
    rdfs:subClassOf ho:FoodPreparation .

ho:prepare_for_brushing_teeth a owl:Class ;
    rdfs:subClassOf ho:HygieneStyling .

ho:prepare_for_work a owl:Class ;
    rdfs:comment "The class with sequence of actions for preparing for work." ;
    rdfs:subClassOf ho:Work .

ho:prepare_go_out a owl:Class ;
    rdfs:comment "added by virtualhome2kg"@en ;
    rdfs:subClassOf ho:GettingReady .

ho:prepare_letter_for_mailing a owl:Class ;
    rdfs:comment """The class with sequence of actions to prepare a letter that will be send \r
for mailing later.""" ;
    rdfs:subClassOf ho:Work .

ho:prepare_pot_of_boiling_water a owl:Class ;
    rdfs:comment "The class with sequence of actions for prepareing pot of boiling water." ;
    rdfs:subClassOf ho:FoodPreparation .

ho:prepare_sandwich a owl:Class ;
    rdfs:comment "The class with sequence of actions for food preparation." ;
    rdfs:subClassOf ho:FoodPreparation .

ho:prepare_sandwitch a owl:Class ;
    rdfs:comment "The class with sequence of actions for preparing a sandwich." ;
    rdfs:subClassOf ho:FoodPreparation .

ho:prepare_sitting a owl:Class ;
    rdfs:subClassOf ho:HouseArrangement .

ho:pretend_tea a owl:Class ;
    rdfs:comment "The class with sequence of actions for pretending that you are drinking tea." ;
    rdfs:subClassOf ho:Other .

ho:print_documents a owl:Class ;
    rdfs:comment "The class with sequence of actions for printing more than one documents." ;
    rdfs:subClassOf ho:Work .

ho:print_out_document a owl:Class ;
    rdfs:comment """The class with sequence of actions to print out a document, no matter \r
what document.""" ;
    rdfs:subClassOf ho:Work .

ho:print_out_papers a owl:Class ;
    rdfs:comment """The class with sequence of actions for printing out papers, no matter \r
what type of paper.""" ;
    rdfs:subClassOf ho:Work .

ho:pull_hair_out_of_drain a owl:Class ;
    rdfs:comment "The class with sequence of actions for pulling the hair out of drain." ;
    rdfs:subClassOf ho:HouseCleaning .

ho:pull_up_carpet a owl:Class ;
    rdfs:comment "The class with sequence of actions for pulling up th carpet, form any room." ;
    rdfs:subClassOf ho:Other .

ho:push_all_chairs_in a owl:Class ;
    rdfs:comment "The class with sequence of actions for pushing all chairs in (under the table, or other place)." ;
    rdfs:subClassOf ho:HouseArrangement .

ho:push_in_desk_chair a owl:Class ;
    rdfs:comment "The class with sequence of actions for pushing in the desk chair." ;
    rdfs:subClassOf ho:Other .

ho:push_in_dining_room_chair a owl:Class ;
    rdfs:comment """The class with sequence of actions for pushing in the dining room chair, \r
under the table or in other place.""" ;
    rdfs:subClassOf ho:Other .

ho:put_alarm_clock_in_bedroom a owl:Class ;
    rdfs:comment """The class with sequence of actions for setting the alarm clock at \r
specific time, which exists in the bedroom.""" ;
    rdfs:subClassOf ho:BedTimeSleep .

ho:put_away_blankets a owl:Class ;
    rdfs:comment "The class with sequence of actions for putting away blankets." ;
    rdfs:subClassOf ho:Other .

ho:put_away_clean_clothes a owl:Class ;
    rdfs:comment "The class with sequence of actions for for putting away clean clothes." ;
    rdfs:subClassOf ho:HouseArrangement .

ho:put_away_clothes a owl:Class ;
    rdfs:comment "The class with sequence of actions for putting away clothes." ;
    rdfs:subClassOf ho:Other .

ho:put_away_dishes a owl:Class ;
    rdfs:comment "The class with sequence of actions for putting away the dishes." ;
    rdfs:subClassOf ho:HouseArrangement .

ho:put_away_groceries a owl:Class ;
    rdfs:comment """The class with sequence of actions for putting away the groceries, not \r
in specific room.""" ;
    rdfs:subClassOf ho:HouseArrangement .

ho:put_away_groceries_from_fridge a owl:Class ;
    rdfs:subClassOf ho:HouseArrangement .

ho:put_away_jackets a owl:Class ;
    rdfs:comment "The class with sequence of actions for putting away the jackets." ;
    rdfs:subClassOf ho:Other .

ho:put_away_keys a owl:Class ;
    rdfs:comment """The class with sequence of actions for putting away keys, in their \r
storing place.""" ;
    rdfs:subClassOf ho:Other .

ho:put_away_shoes a owl:Class ;
    rdfs:comment "The class with sequence of actions for putting away the shoes." ;
    rdfs:subClassOf ho:Other .

ho:put_away_toys a owl:Class ;
    rdfs:comment "The class with sequence of actions for putting away the toys." ;
    rdfs:subClassOf ho:Other .

ho:put_clothes_away a owl:Class ;
    rdfs:comment "The class with sequence of actions for putting clothes away." ;
    rdfs:subClassOf ho:Other .

ho:put_dishes_away a owl:Class ;
    rdfs:comment """The class with sequence of actions for putting dishes away from any \r
place.""" ;
    rdfs:subClassOf ho:HouseArrangement .

ho:put_down_bags a owl:Class ;
    rdfs:comment "The class with sequence of actions for putting down bags, in any room." ;
    rdfs:subClassOf ho:Other .

ho:put_down_decoration a owl:Class ;
    rdfs:comment """The class with sequence of actions for putting down decoration, on the \r
floor or table.""" ;
    rdfs:subClassOf ho:HouseArrangement .

ho:put_dvds_on_shelves a owl:Class ;
    rdfs:comment """The class with sequence of actions for putting the dvds on shelves\r
.""" ;
    rdfs:subClassOf ho:HouseArrangement .

ho:put_food_in_fridge a owl:Class ;
    rdfs:comment "added by virtualhome2kg"@en ;
    rdfs:subClassOf ho:HouseArrangement .

ho:put_groceries_in_fridge a owl:Class ;
    rdfs:comment """Class with sequences that show how to put groceries and other object in \r
the fridge.""" ;
    rdfs:subClassOf ho:HouseArrangement .

ho:put_in_chair a owl:Class ;
    rdfs:comment """The class with sequence of actions for putting in the chair or chairs in \r
any room.""" ;
    rdfs:subClassOf ho:Other .

ho:put_mail_away a owl:Class ;
    rdfs:comment """The class with sequence of actions for putiing mails away, in a specific \r
place.""" ;
    rdfs:subClassOf ho:HouseArrangement .

ho:put_mail_in_mail_organizer a owl:Class ;
    rdfs:comment "The class with sequence of actions for puttin mail in mail organizer." ;
    rdfs:subClassOf ho:HouseArrangement .

ho:put_new_books_in_shelves a owl:Class ;
    rdfs:comment """The class with sequence of actions for putting new books in shelves, \r
from another place.""" ;
    rdfs:subClassOf ho:HouseArrangement .

ho:put_on_coat a owl:Class ;
    rdfs:comment "The class with sequence of actions for putting on your coat." ;
    rdfs:subClassOf ho:HygieneStyling .

ho:put_on_coat_and_shoes a owl:Class ;
    rdfs:comment "The class with sequence of actions for putiing on coat and shoes." ;
    rdfs:subClassOf ho:HygieneStyling .

ho:put_on_foundation a owl:Class ;
    rdfs:comment "The class with sequence of actions for putting on a foundation." ;
    rdfs:subClassOf ho:HygieneStyling .

ho:put_on_glasses a owl:Class ;
    rdfs:comment "The class with sequence of actions for putting your glasses on." ;
    rdfs:subClassOf ho:HygieneStyling .

ho:put_on_purse_put_keys_and_lucky_charms_in_pockets_leave_home a owl:Class ;
    rdfs:comment """The class with sequence of actions for putting on purse, putting keys \r
and lucjy charm in pockets, and leave home.""" ;
    rdfs:subClassOf ho:Other .

ho:put_on_your_shoes a owl:Class ;
    rdfs:comment """The class with sequence of actions for putiing on your shoes, in any \r
room.""" ;
    rdfs:subClassOf ho:HygieneStyling .

ho:put_out_flowers a owl:Class ;
    rdfs:comment "The class with sequence of actions for putting out flowers on the balcony, or some external place of the house." ;
    rdfs:subClassOf ho:Other .

ho:put_shoes_and_coats a owl:Class ;
    rdfs:comment "The class with sequence of actions for putting shoes and coats." ;
    rdfs:subClassOf ho:HygieneStyling .

ho:put_shoes_in_shoe_rack a owl:Class ;
    rdfs:comment "The class with sequence of actions for putting the shoes in shoe rack, wherever the shoe rack is." ;
    rdfs:subClassOf ho:HouseArrangement .

ho:put_slippers_in_closet a owl:Class ;
    rdfs:comment """The class with sequence of actions for putting slippers in closet, in \r
any room the closet is.""" ;
    rdfs:subClassOf ho:HouseArrangement .

ho:put_them_to_sleep a owl:Class ;
    rdfs:comment "The class with sequence of actions for putting them to sleep." ;
    rdfs:subClassOf ho:BedTimeSleep .

ho:put_toys_away a owl:Class ;
    rdfs:comment """The class with sequence of actions for putting the toys away, that \r
belong to childeren or your own.""" ;
    rdfs:subClassOf ho:HouseArrangement .

ho:put_umbrella_away a owl:Class ;
    rdfs:comment """The class with sequence of actions for putting the umbrella away, in any \r
place.""" ;
    rdfs:subClassOf ho:Other .

ho:put_up_coat a owl:Class ;
    rdfs:comment """<p style="margin-top: 0">\r
      The class with sequence of actions for putting up coat.\r
    </p>""" ;
    rdfs:subClassOf ho:HygieneStyling .

ho:put_up_decoration a owl:Class ;
    rdfs:comment "The class with sequence of actions for putting up decoration." ;
    rdfs:subClassOf ho:Other .

ho:put_up_feet a owl:Class ;
    rdfs:comment "The class with sequence of actions for putting up your feet, in any place and room." ;
    rdfs:subClassOf ho:Other .

ho:put_up_jacket a owl:Class ;
    rdfs:comment "The class with sequence of actions for putting up a jacket, in any room." ;
    rdfs:subClassOf ho:Other .

ho:put_up_towel a owl:Class ;
    rdfs:comment """The class with sequence of actions for putting up towel, in any room on \r
you.""" ;
    rdfs:subClassOf ho:Other .

ho:put_washed_clothes_in_almirah a owl:Class ;
    rdfs:comment "The class with sequence of actions for putting washed clothes in almirah." ;
    rdfs:subClassOf ho:HouseArrangement .

ho:rain_welcome a owl:Class ;
    rdfs:comment """he class with sequence of actions for raining welcome (comming inside \r
the house, after rain).""" ;
    rdfs:subClassOf ho:Other .

ho:raise_blinds a owl:Class ;
    rdfs:comment """The class with sequence of actions for raising blinds, from any window in any room.\r
    </p>""" ;
    rdfs:subClassOf ho:Other .

ho:re_arrange_office a owl:Class ;
    rdfs:comment """The class with sequence of actions for re arranging office, cleaning or \r
sorting items, etc.""" ;
    rdfs:subClassOf ho:HouseArrangement .

ho:read_bedtime_story a owl:Class ;
    rdfs:subClassOf ho:BedTimeSleep .

ho:read_book a owl:Class ;
    rdfs:comment "Class which contains sequence of action, about how to read of a book." ;
    rdfs:subClassOf ho:Leisure .

ho:read_magazine a owl:Class ;
    rdfs:comment """The class with sequence of actions for reading a magazine (not a \r
newspaper).""" ;
    rdfs:subClassOf ho:Leisure .

ho:read_news a owl:Class ;
    rdfs:comment """The class with sequence of actions for reading news (either from a \r
newspaper, either from the internet).""" ;
    rdfs:subClassOf ho:Leisure .

ho:read_newspaper a owl:Class ;
    rdfs:comment "The class with sequence of actions for reading a newspaper." ;
    rdfs:subClassOf ho:Leisure .

ho:read_on_sofa a owl:Class ;
    rdfs:comment """The class with sequence of actions reading womehting (newspaper, or \r
book or magazine), while on the sofa.""" ;
    rdfs:subClassOf ho:Leisure .

ho:read_paper a owl:Class ;
    rdfs:comment "The class with sequence of actions for reading some kind of paper." ;
    rdfs:subClassOf ho:Work .

ho:read_text_message a owl:Class ;
    rdfs:comment """The class with sequence of actions for reading text message, form the \r
phone, or computer.""" ;
    rdfs:subClassOf ho:Other .

ho:read_textbook a owl:Class ;
    rdfs:subClassOf ho:Work .

ho:read_them_bedtime_story a owl:Class ;
    rdfs:comment """The class with sequence of actions for reading to someone lese a bedtime \r
story.""" ;
    rdfs:subClassOf ho:BedTimeSleep .

ho:read_to_child a owl:Class ;
    rdfs:comment "The class with sequence of actions for readin to your child in any room." ;
    rdfs:subClassOf ho:SocialInteraction .

ho:read_yourself_to_sleep a owl:Class ;
    rdfs:comment """The class with sequence of actions for reading and falling to sleep \r
while reading.""" ;
    rdfs:subClassOf ho:Leisure .

ho:rearrange_photo_frames a owl:Class ;
    rdfs:comment "The class with sequence of actions for rearranging photo frames." ;
    rdfs:subClassOf ho:HouseArrangement .

ho:receive_credit_card a owl:Class ;
    rdfs:comment "The class with sequence of actions for receiving a credit card." ;
    rdfs:subClassOf ho:Other .

ho:recycle_items a owl:Class ;
    rdfs:comment "The class with sequence of actions for recycling items." ;
    rdfs:subClassOf ho:Other .

ho:relax a owl:Class ;
    rdfs:comment "The class with sequence of actions for relaxing." ;
    rdfs:subClassOf ho:Leisure .

ho:relax_on_bed a owl:Class ;
    rdfs:subClassOf ho:Leisure .

ho:relax_on_sofa a owl:Class ;
    rdfs:comment "This class contains sequence of actions on how you can relax on a sofa." ;
    rdfs:subClassOf ho:Leisure .

ho:relax_on_sofa_while_watching_television a owl:Class ;
    rdfs:subClassOf ho:Leisure .

ho:replace_toothpaste a owl:Class ;
    rdfs:comment """The class with sequence of actions for replacing the toohtpaste in any \r
room.""" ;
    rdfs:subClassOf ho:HouseArrangement .

ho:replace_towel a owl:Class ;
    rdfs:comment "The class with sequence of actions for replacing a towel, from any room." ;
    rdfs:subClassOf ho:Other .

ho:research a owl:Class ;
    rdfs:comment "The class with sequence of actions for performing research." ;
    rdfs:subClassOf ho:Work .

ho:restock a owl:Class ;
    rdfs:comment "The class with sequence of actions for restocking, any place." ;
    rdfs:subClassOf ho:Other .

ho:return_from_store a owl:Class ;
    rdfs:comment "The class with sequence of actions for returning from the store." ;
    rdfs:subClassOf ho:Other .

ho:return_phone_calls a owl:Class ;
    rdfs:comment """The class with sequence of actions for returning phone calls, either \r
from your cell phone or home phone.""" ;
    rdfs:subClassOf ho:Other .

ho:rinse_toothbrush a owl:Class ;
    rdfs:subClassOf ho:HygieneStyling .

ho:rotate_stock_in_refrigerator a owl:Class ;
    rdfs:comment "The class with sequence of actions for rotating stock in Refrigerator." ;
    rdfs:subClassOf ho:HouseArrangement .

ho:run_with_disorientation a owl:Class ;
    rdfs:subClassOf ho:Abnormal .

ho:say_goodbye a owl:Class ;
    rdfs:comment "The class with sequence of actions for greeding by saying goodbye." ;
    rdfs:subClassOf ho:SocialInteraction .

ho:say_goodbye_to_guests_leaving a owl:Class ;
    rdfs:comment "The class with sequence of actions for saying goodbye to guests leaving." ;
    rdfs:subClassOf ho:SocialInteraction .

ho:scrub_bottom_of_feet a owl:Class ;
    rdfs:comment "The class with sequence of actions for scrubbing just the bottom of your feet." ;
    rdfs:subClassOf ho:HygieneStyling .

ho:scrub_face a owl:Class ;
    rdfs:comment "The class with sequence of actions for scrubing you face." ;
    rdfs:subClassOf ho:HygieneStyling .

ho:scrub_toilet a owl:Class ;
    rdfs:comment "The class with sequence of actions for scrubing the toilet." ;
    rdfs:subClassOf ho:HouseCleaning .

ho:scrubbing_living_room_tile_floor_is_once_week_activity_for_me a owl:Class ;
    rdfs:comment "The class with sequence of actions for scrubbing living room tile floor is once a week activity for me." ;
    rdfs:subClassOf ho:HouseCleaning .

ho:send__email a owl:Class ;
    rdfs:comment "The class with sequence of actions for sending an email." ;
    rdfs:subClassOf ho:Work .

ho:sent_email a owl:Class ;
    rdfs:comment "The class with sequence of actions to send a email." ;
    rdfs:subClassOf ho:Work .

ho:serve_breakfast a owl:Class ;
    rdfs:comment "The class with sequence of actions for serving breakfast, in any room." ;
    rdfs:subClassOf ho:Other .

ho:serve_cookies a owl:Class ;
    rdfs:comment "The class with sequence of actions for serving cookies, for any occasion." ;
    rdfs:subClassOf ho:Other .

ho:serve_food a owl:Class ;
    rdfs:comment "The class with sequence of actions for serving the food in any room." ;
    rdfs:subClassOf ho:Other .

ho:serve_hors_doeurves_to_entering_guests_at_cocktail_party a owl:Class ;
    rdfs:comment "The class with sequence of actions for srving hors doeurves to entering guest at cocktail party." ;
    rdfs:subClassOf ho:SocialInteraction .

ho:serve_meal a owl:Class ;
    rdfs:comment "The class with sequence of actions for serving meal in any room." ;
    rdfs:subClassOf ho:Other .

ho:set_mail_on_table a owl:Class ;
    rdfs:comment "The class with sequence of actions for setting the mail on the table, for eating." ;
    rdfs:subClassOf ho:Other .

ho:set_out_some_snacks_for_toddler a owl:Class ;
    rdfs:comment "The class with sequence of actions for setting out some snacks for toddler." ;
    rdfs:subClassOf ho:Other .

ho:set_up_buffet_area a owl:Class ;
    rdfs:comment "The class with sequence of actions for setting up the buffet area." ;
    rdfs:subClassOf ho:HouseArrangement .

ho:set_up_table a owl:Class ;
    rdfs:comment "Class with sequences about how to perform the set up of a dinner, kitchen table." ;
    rdfs:subClassOf ho:HouseArrangement .

ho:set_up_tv a owl:Class ;
    rdfs:comment "The class with sequence of actions for seeting up the TV." ;
    rdfs:subClassOf ho:Other .

ho:settle_in a owl:Class ;
    rdfs:comment "The class with sequence of actions for settling in the house." ;
    rdfs:subClassOf ho:Other .

ho:sew_button a owl:Class ;
    rdfs:comment """The class with sequence of actions for sewing the button, from any \r
remote control.""" ;
    rdfs:subClassOf ho:Other .

ho:shampoo_hair a owl:Class ;
    rdfs:comment "The class with sequence of actions for shampooing your hair." ;
    rdfs:subClassOf ho:HygieneStyling .

ho:shoe_removal a owl:Class ;
    rdfs:comment "The class with sequence of actions for removing your shoes in any room." ;
    rdfs:subClassOf ho:Other .

ho:shop a owl:Class ;
    rdfs:comment """The class with sequence of actions for shopping either by calling, or \r
from the internet (shopping from household environment).""" ;
    rdfs:subClassOf ho:Other .

ho:shoulder_stretch a owl:Class ;
    rdfs:subClassOf ho:PhysicalActivity .

ho:shred_receipts a owl:Class ;
    rdfs:comment "The class with sequence of actions for shred of receipts." ;
    rdfs:subClassOf ho:HouseCleaning .

ho:shredding a owl:Class ;
    rdfs:comment "The class with sequence of actions for shredding any object in any room." ;
    rdfs:subClassOf ho:Other .

ho:shut_front_door a owl:Class ;
    rdfs:comment "The class with sequence of actions for shutting front door (door of main entrance)." ;
    rdfs:subClassOf ho:Other .

ho:shut_off_alarm a owl:Class ;
    rdfs:comment "The class with sequence of actions for shutting of the alarm in any room." ;
    rdfs:subClassOf ho:Other .

ho:sing_karaoke a owl:Class ;
    rdfs:comment "The class with sequence of actions for singing at the karoke." ;
    rdfs:subClassOf ho:Leisure .

ho:sing_song a owl:Class ;
    rdfs:comment "The class with sequence of actions for singing songs." ;
    rdfs:subClassOf ho:Leisure .

ho:sit_in_chair a owl:Class ;
    rdfs:comment """The class with sequence of actions for sitting in the chair, in any type \r
of chair in any room.""" ;
    rdfs:subClassOf ho:Other .

ho:sit_quietly a owl:Class ;
    rdfs:comment "The class with sequence of actions for sitting quetly, in any room." ;
    rdfs:subClassOf ho:Other .

ho:sleep a owl:Class ;
    rdfs:comment "The class with sequence of actions for sleeping." ;
    rdfs:subClassOf ho:BedTimeSleep .

ho:slice_apple a owl:Class ;
    rdfs:comment "The class with sequence of actions for slicing an apple." ;
    rdfs:subClassOf ho:FoodPreparation .

ho:social_media__checks a owl:Class ;
    rdfs:comment """The class with sequence of actions for chencking your social media \r
applications.""" ;
    rdfs:subClassOf ho:Leisure .

ho:social_media_checks a owl:Class ;
    rdfs:subClassOf ho:Leisure .

ho:sort_and_fold_laundry a owl:Class ;
    rdfs:comment "The class with sequence of actions for sorting and folding laundry." ;
    rdfs:subClassOf ho:HouseCleaning .

ho:sort_clothing_and_care_for_it a owl:Class ;
    rdfs:comment "The class with sequence of actions for sorting clothing in specific order." ;
    rdfs:subClassOf ho:HouseArrangement .

ho:sort_laundry a owl:Class ;
    rdfs:comment "The class with sequence of actions for sorting laundry by category." ;
    rdfs:subClassOf ho:HouseArrangement .

ho:sort_mail a owl:Class ;
    rdfs:comment """The class with sequence of actions for sorting mail, in any desired \r
order.""" ;
    rdfs:subClassOf ho:Other .

ho:speaking_on_headset_in_skype_or_some_form_of_voip_for_business_call a owl:Class ;
    rdfs:comment """The class with sequence of actions for speaking on headset in skype or \r
some form of voip for business call.""",
        "The class with sequence of actions for speaking on headset in skype or some form of voip for business call." ;
    rdfs:subClassOf ho:SocialInteraction,
        ho:Work .

ho:spend_family_time_playing_games a owl:Class ;
    rdfs:comment "The class with sequence of actions for spending family time playing games, videogames of any other games." ;
    rdfs:subClassOf ho:SocialInteraction .

ho:spread_table_with_appropriate_supplies a owl:Class ;
    rdfs:comment """The class with sequence of actions for spreading the table with \r
approproate supplies.""" ;
    rdfs:subClassOf ho:Other .

ho:squat_jumps a owl:Class ;
    rdfs:subClassOf ho:PhysicalActivity .

ho:squats a owl:Class ;
    rdfs:subClassOf ho:PhysicalActivity .

ho:squeeze_lemon a owl:Class ;
    rdfs:comment "The class with sequence of actions for squezing a lemon." ;
    rdfs:subClassOf ho:FoodPreparation .

ho:stand_on_coffee_table a owl:Class ;
    rdfs:subClassOf ho:Abnormal .

ho:start_computer a owl:Class ;
    rdfs:comment """The class with sequence of actions for starting your computer, either \r
laptop or personal computer.""" ;
    rdfs:subClassOf ho:Other .

ho:steam_mop_floor a owl:Class ;
    rdfs:comment "The class with sequence of actions for steaming mop floor." ;
    rdfs:subClassOf ho:HouseCleaning .

ho:story_reading_time a owl:Class ;
    rdfs:comment "The class with sequence of actions for story reading time, in any room." ;
    rdfs:subClassOf ho:SocialInteraction .

ho:straddle_splits a owl:Class ;
    rdfs:subClassOf ho:PhysicalActivity .

ho:straighten_bookshelf a owl:Class ;
    rdfs:comment """The class with sequence of actions for straightening the bookself, in \r
any room.""" ;
    rdfs:subClassOf ho:Other .

ho:straighten_magazines a owl:Class ;
    rdfs:comment """The class with sequence of actions for straighten magaziens that are \r
placed in a folder or on a surface.""" ;
    rdfs:subClassOf ho:HouseArrangement .

ho:straighten_paintings_on_wall a owl:Class ;
    rdfs:comment """The class with sequence of actions for straightening paintings on wall \r
(only painting not pictures).""" ;
    rdfs:subClassOf ho:HouseArrangement .

ho:straighten_pictures_on_wall a owl:Class ;
    rdfs:comment "The class with sequence of actions for straighten pictures on wall, in any room." ;
    rdfs:subClassOf ho:HouseArrangement .

ho:string_green_beans a owl:Class ;
    rdfs:comment """The class with sequence of actions for stringing green beans, in any \r
room.""" ;
    rdfs:subClassOf ho:Other .

ho:study a owl:Class ;
    rdfs:comment "The class with sequence of actions for studying, no matter on what (computer, paper)." ;
    rdfs:subClassOf ho:Work .

ho:study_bible a owl:Class ;
    rdfs:comment "The class with sequence of actions for studying the biblie." ;
    rdfs:subClassOf ho:Work .

ho:style_hair a owl:Class ;
    rdfs:comment "The class with sequence of actions for styling your hair." ;
    rdfs:subClassOf ho:HygieneStyling .

ho:surf_internet a owl:Class ;
    rdfs:comment "The class with sequence of actions for surfing the internet." ;
    rdfs:subClassOf ho:Leisure .

ho:surf_net a owl:Class ;
    rdfs:comment "The class with sequence of actions for surfing the net." ;
    rdfs:subClassOf ho:Leisure .

ho:surf_web_for_money_legitimate_making_opportunities a owl:Class ;
    rdfs:comment """The class with sequence of actions for searching in the internet for \r
legitimate maikng opportunities.""" ;
    rdfs:subClassOf ho:Work .

ho:sweep_and_wipe_table_off_with_rag a owl:Class ;
    rdfs:comment """The class with sequence of actions for sweeping and wiping a table off \r
with a rag.""" ;
    rdfs:subClassOf ho:HouseCleaning .

ho:sweep_entrance_hall a owl:Class ;
    rdfs:comment "The class with sequence of actions on how to sweep the entrance hall." ;
    rdfs:subClassOf ho:HouseCleaning .

ho:sweep_floor a owl:Class ;
    rdfs:comment "The class with sequence of actions for house cleaning." ;
    rdfs:subClassOf ho:HouseCleaning .

ho:sweep_hallway_please a owl:Class ;
    rdfs:comment """he class with sequence of actions to sweep the hallway after you got \r
the verbal token "please".""" ;
    rdfs:subClassOf ho:HouseCleaning .

ho:switch_on_lamp a owl:Class ;
    rdfs:comment "The class with sequence of actions for switching on lamp, in any room." ;
    rdfs:subClassOf ho:Other .

ho:tabletop_game a owl:Class ;
    rdfs:comment """The class with sequence of actions for playin tabletop games (board \r
games).""" ;
    rdfs:subClassOf ho:Leisure .

ho:take_a_nap a owl:Class ;
    rdfs:subClassOf ho:BedTimeSleep .

ho:take_bath a owl:Class ;
    rdfs:comment "Class with seqeunces on how you can take a bath, and clean yourself (not a shower)." ;
    rdfs:subClassOf ho:HygieneStyling .

ho:take_coat a owl:Class ;
    rdfs:comment """The class with sequence of actions for taking the coat, and place it \r
somewhere.""" ;
    rdfs:subClassOf ho:Other .

ho:take_dishes_out_of_dishwasher a owl:Class ;
    rdfs:comment "The class with sequence of actions for taking dishes out of dishwasher." ;
    rdfs:subClassOf ho:HouseArrangement .

ho:take_jacket_off a owl:Class ;
    rdfs:comment "The class with sequence of actions for taking your jacket off." ;
    rdfs:subClassOf ho:HygieneStyling .

ho:take_nap a owl:Class ;
    rdfs:comment "A class with sequences on how to go take a small nap." ;
    rdfs:subClassOf ho:BedTimeSleep .

ho:take_of_outerwear a owl:Class ;
    rdfs:comment "The class with sequence of actions for taking of outerwear." ;
    rdfs:subClassOf ho:Other .

ho:take_off_clock a owl:Class ;
    rdfs:subClassOf ho:HouseArrangement .

ho:take_off_coat a owl:Class ;
    rdfs:comment "The class with sequence of actions for taking of your coat." ;
    rdfs:subClassOf ho:HygieneStyling .

ho:take_off_outerwear a owl:Class ;
    rdfs:comment "The class with sequence of actions for getting ready." ;
    rdfs:subClassOf ho:GettingReady .

ho:take_off_shoes a owl:Class ;
    rdfs:comment """Class with seqeunces on how to take off your shoes after work, or before \r
getting to bed, or watch tv.""" ;
    rdfs:subClassOf ho:HygieneStyling .

ho:take_off_shoes_and_hang_up_coat a owl:Class ;
    rdfs:comment "The class with sequence of actions for hanging up your coat." ;
    rdfs:subClassOf ho:HygieneStyling .

ho:take_shoes_off a owl:Class ;
    rdfs:comment "The class with sequence of actions for taking yur shoes off." ;
    rdfs:subClassOf ho:HygieneStyling .

ho:take_shower a owl:Class ;
    rdfs:comment """Class with seqeunces of action on how to take a shower (not a bath)\r
.""" ;
    rdfs:subClassOf ho:HygieneStyling .

ho:tale_off_shoes a owl:Class ;
    rdfs:comment "The class with sequence of actions for taling of your own shoes." ;
    rdfs:subClassOf ho:HygieneStyling .

ho:talk_on_phone a owl:Class ;
    rdfs:comment """The class with sequence of actions for talking on phone, either cell \r
phone or phone at home.""" ;
    rdfs:subClassOf ho:SocialInteraction .

ho:talk_to_kids a owl:Class ;
    rdfs:comment "The class with sequence of actions for talking to kids in any room." ;
    rdfs:subClassOf ho:SocialInteraction .

ho:talk_with_friends a owl:Class ;
    rdfs:comment """The class with sequence of actions for talking to your friend, no matter \r
the genre.""" ;
    rdfs:subClassOf ho:SocialInteraction .

ho:talk_with_guest a owl:Class ;
    rdfs:comment "The class with sequence of actions for talking to guest." ;
    rdfs:subClassOf ho:SocialInteraction .

ho:talk_with_your_child_about_their_day a owl:Class ;
    rdfs:comment """The class with sequence of actions for talking with your child about \r
their day.""" ;
    rdfs:subClassOf ho:SocialInteraction .

ho:tax_filing a owl:Class ;
    rdfs:comment "The class with sequence of actions for filling your taxes." ;
    rdfs:subClassOf ho:Work .

ho:teach_them_to_make_their_bed a owl:Class ;
    rdfs:comment """The class with sequence of actions for teaching them (other persons), to \r
make their beds.""" ;
    rdfs:subClassOf ho:Other .

ho:tell_jokes a owl:Class ;
    rdfs:comment "The class with sequence of actions for telling jokes to any individual." ;
    rdfs:subClassOf ho:SocialInteraction .

ho:text_friend a owl:Class ;
    rdfs:comment "The class with sequence of actions for texting a friend." ;
    rdfs:subClassOf ho:SocialInteraction .

ho:text_friends_while_sitting_on_couch a owl:Class ;
    rdfs:comment """The class with sequence of actions for texting a frined while you are \r
sitting on the couch.""" ;
    rdfs:subClassOf ho:SocialInteraction .

ho:thanksgiving a owl:Class ;
    rdfs:comment "The class with sequence of actions for thanksgiving." ;
    rdfs:subClassOf ho:SocialInteraction .

ho:throw_away_newspaper a owl:Class ;
    rdfs:comment """The class with sequence of actions for throwing away newspaper, in the \r
garbage can, or elsewhere.""" ;
    rdfs:subClassOf ho:Other .

ho:throw_away_paper a owl:Class ;
    rdfs:comment """The class with sequence of actions for throwing away paper, in the \r
garbage that could be in any room.""" ;
    rdfs:subClassOf ho:Other .

ho:throw_in_the_garbage a owl:Class ;
    rdfs:comment "added by virtualhome2kg"@en ;
    rdfs:subClassOf ho:HouseCleaning .

ho:throw_shoes a owl:Class ;
    rdfs:comment "The class with sequence of actions for throwing away shoes, in any room." ;
    rdfs:subClassOf ho:Other .

ho:throw_trash a owl:Class ;
    rdfs:subClassOf ho:HouseArrangement .

ho:tidy a owl:Class ;
    rdfs:comment "The class with sequence of actions for tiding anything." ;
    rdfs:subClassOf ho:Other .

ho:toast_bread a owl:Class ;
    rdfs:comment """The class with sequence of actions for toasting the bread (to prepare a \r
toast or something else).""" ;
    rdfs:subClassOf ho:FoodPreparation .

ho:toilet a owl:Class ;
    rdfs:comment "The class with sequence of actions for going to the toilet." ;
    rdfs:subClassOf ho:HygieneStyling .

ho:transcribe_what_i_say a owl:Class ;
    rdfs:comment "The class with sequence of actions for trancribe (or copy) the words that I say." ;
    rdfs:subClassOf ho:Work .

ho:trick_or_treat a owl:Class ;
    rdfs:comment "The class with sequence of actions for trick or treat." ;
    rdfs:subClassOf ho:SocialInteraction .

ho:try_yourself_off a owl:Class ;
    rdfs:comment """The class with sequence of actions for trying yourself off, with any \r
activity in any room.""" ;
    rdfs:subClassOf ho:Other .

ho:tuck_kids_in_bed a owl:Class ;
    rdfs:comment "A class with sequences to put the kids in bed for sleep, or tell a story." ;
    rdfs:subClassOf ho:SocialInteraction .

ho:tummy_time a owl:Class ;
    rdfs:comment "The class with sequence of actions for tummy time." ;
    rdfs:subClassOf ho:Other .

ho:turking a owl:Class ;
    rdfs:comment "The class with sequence of actions for turking." ;
    rdfs:subClassOf ho:Other .

ho:turn_light_off a owl:Class ;
    rdfs:comment """The class with sequence of actions for  turning off the light form any \r
room.""" ;
    rdfs:subClassOf ho:Other .

ho:turn_night_light_on a owl:Class ;
    rdfs:comment "The class with sequence of actions for turning the night light on." ;
    rdfs:subClassOf ho:HouseArrangement .

ho:turn_off_light a owl:Class ;
    rdfs:comment "The class with sequence of actions for turning off the lights." ;
    rdfs:subClassOf ho:HouseArrangement .

ho:turn_off_tv a owl:Class ;
    rdfs:comment "The class with sequence of actions for turning off the TV." ;
    rdfs:subClassOf ho:Leisure .

ho:turn_on_computer a owl:Class ;
    rdfs:comment """The class with sequence of actions for turning on a computer (laptop, or \r
personal computer).""" ;
    rdfs:subClassOf ho:Other .

ho:turn_on_light a owl:Class ;
    rdfs:comment """A class with sequences on how to turn on the lights from different \r
rooms, and different scenaria such as holding other objects or having to \r
stand up from bed.""" ;
    rdfs:subClassOf ho:HouseArrangement,
        ho:Other .

ho:turn_on_lights a owl:Class ;
    rdfs:comment """The class with sequence of actions for turning on the lights more than \r
one.""" ;
    rdfs:subClassOf ho:Other .

ho:turn_on_radio a owl:Class ;
    rdfs:comment """The class with sequence of actions for turning on the radio (just \r
turning on).\r
    </p>""" ;
    rdfs:subClassOf ho:Leisure .

ho:turn_on_tv a owl:Class ;
    rdfs:comment "The class with sequence of actions on hoe to turn on the TV (just turn on tv, not other actions)." ;
    rdfs:subClassOf ho:Leisure .

ho:turn_on_tv_with_remote a owl:Class ;
    rdfs:comment "The class with sequence of actions for watching tv while using remote control." ;
    rdfs:subClassOf ho:Leisure .

ho:type_up_document a owl:Class ;
    rdfs:comment "The class with sequence of actions for typing up a document." ;
    rdfs:subClassOf ho:Work .

ho:unload_dishwasher a owl:Class ;
    rdfs:comment "The class with sequence of actions for unloadinf the dishwasher." ;
    rdfs:subClassOf ho:HouseArrangement .

ho:unload_various_items_from_pockets_and_place_them_in_bowl_on_table a owl:Class ;
    rdfs:comment """The class with sequence of actions for unloading various itmes form \r
pockets and place them in bowl on table.""" ;
    rdfs:subClassOf ho:HouseArrangement .

ho:update_address_book a owl:Class ;
    rdfs:comment """The class with sequence of actions that are neede to update your address \r
book.""" ;
    rdfs:subClassOf ho:Work .

ho:use_bathroom a owl:Class ;
    rdfs:comment """The class with sequence of actions for using the bathroom, the whole \r
room.""" ;
    rdfs:subClassOf ho:HygieneStyling .

ho:use_computer a owl:Class ;
    rdfs:comment "Class wih sequences on how to perform general task with a computer." ;
    rdfs:subClassOf ho:Work .

ho:use_laptop a owl:Class ;
    rdfs:comment """The class with sequence of actions for using your laptop, variety of \r
functions.""" ;
    rdfs:subClassOf ho:Other .

ho:use_phone a owl:Class ;
    rdfs:subClassOf ho:Leisure .

ho:use_restroom a owl:Class ;
    rdfs:comment "The class with sequence of actions for using the restroom." ;
    rdfs:subClassOf ho:HygieneStyling .

ho:use_smartphone a owl:Class ;
    rdfs:subClassOf ho:Leisure .

ho:use_toilet a owl:Class ;
    rdfs:comment "The class with sequence of actions for using the toilet." ;
    rdfs:subClassOf ho:HygieneStyling .

ho:vacuum_carpet a owl:Class ;
    rdfs:comment "The class with sequence of actions for vacuum the carpet." ;
    rdfs:subClassOf ho:HouseCleaning .

ho:visit a owl:Class ;
    rdfs:comment "The class with sequence of actions for visitng someone elses house." ;
    rdfs:subClassOf ho:SocialInteraction .

ho:visit_neighbors a owl:Class ;
    rdfs:comment "The class with sequence of actions for visitng neighbors." ;
    rdfs:subClassOf ho:SocialInteraction .

ho:visit_with_friends_while_engaging_in_games a owl:Class ;
    rdfs:comment "The class with sequence of actions for visiting friends while engaging in games." ;
    rdfs:subClassOf ho:Other .

ho:wake_kids_up a owl:Class ;
    rdfs:comment "The class with sequence of actions for waking kids up from sleep." ;
    rdfs:subClassOf ho:SocialInteraction .

ho:wake_me_up a owl:Class ;
    rdfs:comment "The class with sequence of actions for telling the system to wake up the user." ;
    rdfs:subClassOf ho:BedTimeSleep .

ho:walk_through a owl:Class ;
    rdfs:comment "The class with sequence of actions for walking through a door." ;
    rdfs:subClassOf ho:Other .

ho:walk_to_room a owl:Class ;
    rdfs:comment "The class with sequence of actions for walking to room, any room." ;
    rdfs:subClassOf ho:Other .

ho:walk_with_memory_loss a owl:Class ;
    rdfs:subClassOf ho:Abnormal .

ho:wash_and_clean_all_crystal_in_china_cabinet a owl:Class ;
    rdfs:comment """The class with sequence of actions for washing and cleaning all crystal \r
in china cabinet.""" ;
    rdfs:subClassOf ho:HouseArrangement .

ho:wash_back a owl:Class ;
    rdfs:comment """The class with sequence of actions for washing back, your own or others \r
back.""" ;
    rdfs:subClassOf ho:Other .

ho:wash_clothes a owl:Class ;
    rdfs:comment "Class with sequences for washing clothes." ;
    rdfs:subClassOf ho:HouseArrangement,
        ho:HouseCleaning .

ho:wash_dining_table a owl:Class ;
    rdfs:comment "The class with sequence of actions for washing dining table." ;
    rdfs:subClassOf ho:Other .

ho:wash_dirty_dishes a owl:Class ;
    rdfs:comment "The class with sequence of actions for washing dirty dishes." ;
    rdfs:subClassOf ho:HouseCleaning .

ho:wash_dishes a owl:Class ;
    rdfs:comment "The class with sequence of actions for washing up dishes, in the general case or getting ready to wash dishes." ;
    rdfs:subClassOf ho:HouseArrangement .

ho:wash_dishes_by_hand a owl:Class ;
    rdfs:comment "The class with sequence of actions for washing yp dishes by hand only." ;
    rdfs:subClassOf ho:HouseArrangement .

ho:wash_dishes_with_dishwasher a owl:Class ;
    rdfs:comment "The class with sequence of actions for washing up dishes with dishwasher." ;
    rdfs:subClassOf ho:HouseArrangement .

ho:wash_face a owl:Class ;
    rdfs:comment "The class with sequence of actions for washing your face." ;
    rdfs:subClassOf ho:HygieneStyling .

ho:wash_fry_pan a owl:Class ;
    rdfs:comment "added by virtualhome2kg"@en ;
    rdfs:subClassOf ho:HouseCleaning .

ho:wash_hair a owl:Class ;
    rdfs:comment "The class with sequence of actions for washing your hair." ;
    rdfs:subClassOf ho:HygieneStyling .

ho:wash_hands a owl:Class ;
    rdfs:comment "The class with sequence of actions for washing your hands." ;
    rdfs:subClassOf ho:HygieneStyling .

ho:wash_monitor a owl:Class ;
    rdfs:comment "The class with sequence of actions for washing a some kind of monitor." ;
    rdfs:subClassOf ho:HouseCleaning .

ho:wash_pillow a owl:Class ;
    rdfs:subClassOf ho:HouseCleaning .

ho:wash_sink a owl:Class ;
    rdfs:comment "The class with sequence of actions for house cleaning." ;
    rdfs:subClassOf ho:HouseCleaning .

ho:wash_table a owl:Class ;
    rdfs:comment "The class with sequence of actions for washing the table." ;
    rdfs:subClassOf ho:HouseCleaning .

ho:wash_teeth a owl:Class ;
    rdfs:comment "The class with sequence of actions for washing teeth (with water for example)." ;
    rdfs:subClassOf ho:HygieneStyling .

ho:watch__horror__movie a owl:Class ;
    rdfs:comment """The class with sequence of actions for watching a horror movie \r
specifically.""" ;
    rdfs:subClassOf ho:Leisure .

ho:watch_fly a owl:Class ;
    rdfs:comment """The class with sequence of actions for watching a fly that has entered a \r
room.""" ;
    rdfs:subClassOf ho:Other .

ho:watch_movie a owl:Class ;
    rdfs:comment "A class about how to watch a movie either on the TV or laptop." ;
    rdfs:subClassOf ho:Leisure .

ho:watch_television a owl:Class ;
    rdfs:subClassOf ho:Leisure .

ho:watch_tv a owl:Class ;
    rdfs:comment "It contains some subclasses on how to watch TV" ;
    rdfs:subClassOf ho:Leisure .

ho:watch_youtube a owl:Class ;
    rdfs:comment "The class with sequence of actions for wathcing YouTube videos." ;
    rdfs:subClassOf ho:Leisure .

ho:water_plants a owl:Class ;
    rdfs:comment "The class with sequence of actions for watering the plants." ;
    rdfs:subClassOf ho:HouseArrangement .

ho:wave_at_people_walking_by_through_window a owl:Class ;
    rdfs:comment """The class with sequence of actions for waving at people walking by \r
through window.""" ;
    rdfs:subClassOf ho:SocialInteraction .

ho:whine a owl:Class ;
    rdfs:comment "The class with sequence of actions for whining in any room." ;
    rdfs:subClassOf ho:Other .

ho:wipe_down_baseboards_please a owl:Class ;
    rdfs:comment "The class with sequence of actions for wipe down baseboards please." ;
    rdfs:subClassOf ho:Other .

ho:wipe_down_counter a owl:Class ;
    rdfs:comment "The class with sequence of actions for wiping down counter, for any domestic machine that has such." ;
    rdfs:subClassOf ho:Other .

ho:wipe_down_sink a owl:Class ;
    rdfs:comment """The class with sequence of actions in order to wipe down sink, only this \r
part of cleaning not all the cleaning procedure.""" ;
    rdfs:subClassOf ho:HouseCleaning .

ho:wipe_feet a owl:Class ;
    rdfs:comment "The class with sequence of actions for wiping your own feet." ;
    rdfs:subClassOf ho:HygieneStyling .

ho:wipe_off_shoes a owl:Class ;
    rdfs:comment "The class with sequence of actions for wiping your shoes off." ;
    rdfs:subClassOf ho:Other .

ho:wipe_room_down_with_lysol a owl:Class ;
    rdfs:comment "The class with sequence of actions for wiping down the room with lysol." ;
    rdfs:subClassOf ho:HouseCleaning .

ho:workout a owl:Class ;
    rdfs:comment """A class with soft physical activity, or exercise, such as weight \r
lifting, workout.""" ;
    rdfs:subClassOf ho:PhysicalActivity .

ho:write_an_email a owl:Class ;
    rdfs:comment "The class with sequence of actions for wrtiting ana email." ;
    rdfs:subClassOf ho:Work .

ho:write_book a owl:Class ;
    rdfs:comment "The class with sequence of actions for writing a book, in any room." ;
    rdfs:subClassOf ho:Other .

ho:write_in_your_diary a owl:Class ;
    rdfs:comment """The class with sequence of actions for writing in your diary, in any \r
room.""" ;
    rdfs:subClassOf ho:Other .

ho:write_letter a owl:Class ;
    rdfs:comment "Class with sequences on how to write a letter." ;
    rdfs:subClassOf ho:Work .

ho:write_notes a owl:Class ;
    rdfs:subClassOf ho:Work .

ho:write_report a owl:Class ;
    rdfs:comment "The class with sequence of actions for writing some kind of report." ;
    rdfs:subClassOf ho:Work .

ho:write_research_paper a owl:Class ;
    rdfs:comment "The class with sequence of actions for writing a research paper." ;
    rdfs:subClassOf ho:Work .

ho:write_research_papers a owl:Class ;
    rdfs:comment """The class with sequence of actions for writing reaseach papers (only \r
research paper).""" ;
    rdfs:subClassOf ho:Work .

ho:write_school_paper a owl:Class ;
    rdfs:comment """The class with sequence of actions writing school papers, it should not \r
be confused with research paper.""" ;
    rdfs:subClassOf ho:Work .

ho:write_story a owl:Class ;
    rdfs:comment """The class with sequence of actions for writing a story, on the computer \r
or on paper.""" ;
    rdfs:subClassOf ho:Other .

ho:write_thank_you_notes a owl:Class ;
    rdfs:comment "The class with sequence of actions to write a thank you note to somebody." ;
    rdfs:subClassOf ho:Work .

ho:yoga a owl:Class ;
    rdfs:comment "The class with sequence of actions for doing yoga." ;
    rdfs:subClassOf ho:PhysicalActivity .

rdf:first a owl:DatatypeProperty .

rdf:rest a owl:DatatypeProperty .

rdf:value a owl:DatatypeProperty .

skos:closeMatch a owl:AnnotationProperty .

time:hasDuration a owl:ObjectProperty ;
    rdfs:range time:Duration .

time:numericDuration a owl:DatatypeProperty ;
    rdfs:range xsd:decimal .

time:unitSecond a owl:NamedIndividual,
        time:TemporalUnit .

time:unitType a owl:ObjectProperty ;
    rdfs:range time:TemporalUnit .

x3do:SFDouble a rdfs:Datatype,
        owl:Class ;
    dcterms:description "SFDouble is a double-precision floating-point type. Array values are optionally separated by commas in XML syntax. See GeoVRML 1.0 Recommended Practice, Section 2.3, Limitations of Single Precision for rationale." ;
    rdfs:subClassOf x3do:X3DField .

x3do:bboxCenter a owl:DatatypeProperty ;
    rdfs:domain x3do:Shape ;
    rdfs:range x3do:SFVec3f .

x3do:bboxSize a owl:DatatypeProperty ;
    rdfs:domain x3do:Shape ;
    rdfs:range x3do:SFVec3f .

:Character a owl:Class ;
    rdfs:subClassOf :Object .

:VirtualHome a owl:Class .

ac:drink a :Action,
        owl:NamedIndividual .

ac:eat a :Action,
        owl:NamedIndividual .

ac:sleep a :Action,
        owl:NamedIndividual .

ac:wakeUp a :Action,
        owl:NamedIndividual .

:bright a :Attribute,
        owl:NamedIndividual .

:cold a :Attribute,
        owl:NamedIndividual .

:dark a :Attribute,
        owl:NamedIndividual .

:deep a :Attribute,
        owl:NamedIndividual .

:heavy a :Attribute,
        owl:NamedIndividual .

:high a :Attribute,
        owl:NamedIndividual .

:hot a :Attribute,
        owl:NamedIndividual .

:isBboxOf a owl:ObjectProperty ;
    rdfs:domain x3do:Shape .

:long a :Attribute,
        owl:NamedIndividual .

:low a :Attribute,
        owl:NamedIndividual .

:previousSituation a owl:ObjectProperty ;
    rdfs:domain :Situation ;
    rdfs:range :Situation ;
    rdfs:subPropertyOf :relatedSituation .

:previousState a owl:ObjectProperty ;
    rdfs:domain :State ;
    rdfs:range :State ;
    rdfs:subPropertyOf :relatedState .

:shallow a :Attribute,
        owl:NamedIndividual .

:short a :Attribute,
        owl:NamedIndividual .

:thick a :Attribute,
        owl:NamedIndividual .

:thin a :Attribute,
        owl:NamedIndividual .

time:Duration a owl:Class ;
    rdfs:subClassOf time:TemporalDuration .

time:TemporalEntity a owl:Class .

:relatedActivity a owl:ObjectProperty ;
    rdfs:domain ho:Activity ;
    rdfs:range ho:Activity .

:relatedEvent a owl:ObjectProperty ;
    rdfs:domain :Event ;
    rdfs:range :Event .

:relatedState a owl:ObjectProperty ;
    rdfs:domain :State ;
    rdfs:range :State .

<http://plod.info/rdf/Episode> a owl:Class .

ho:object a owl:ObjectProperty ;
    rdfs:domain :Event ;
    rdfs:range :Object .

time:TemporalDuration a owl:Class .

time:TemporalUnit a owl:Class .

x3do:SFVec3f a rdfs:Datatype,
        owl:Class ;
    dcterms:description "SFVec3d is a 3-tuple triplet of SFDouble values. See GeoVRML 1.0 Recommended Practice, Section 2.3, Limitations of Single Precision. Hint: SFVec3d can be used to specify a georeferenced 3D coordinate. Warning: comma characters within singleton values do not pass strict XML validation." ;
    rdfs:subClassOf x3do:X3DField .

x3do:X3DField a owl:Class ;
    rdfs:comment "X3DField is the abstract field type from which all single-valued field types are derived." .

:Unit a owl:Class .

:action a owl:ObjectProperty ;
    rdfs:domain :Event ;
    rdfs:range :Action .

:hasEvent a owl:ObjectProperty ;
    rdfs:domain ho:Activity ;
    rdfs:range :Event .

:relatedSituation a owl:ObjectProperty ;
    rdfs:domain :Situation ;
    rdfs:range :Situation .

ho:GettingReady a owl:Class ;
    rdfs:comment """Class with sequences for getting ready to go to work, or getting ready \r
o perform a task outside the home, or even a procedure that needs prior \r
preparation.""" ;
    rdfs:subClassOf ho:Activity .

:relatedShape a owl:ObjectProperty ;
    rdfs:domain x3do:Shape ;
    rdfs:range x3do:Shape .

:Object a owl:Class .

:Situation a owl:Class ;
    rdfs:comment "The class which describes the situation of the entire home at a certain moment." .

:State a owl:Class .

ho:PhysicalActivity a owl:Class ;
    rdfs:comment "Class with sequences for exercise and different physical activities." ;
    rdfs:subClassOf ho:Activity .

ho:BedTimeSleep a owl:Class ;
    rdfs:comment """Class with sequences for getting ready for the bed, or get ready for \r
sleep, or even put the kids to sleep\r
.""" ;
    rdfs:subClassOf ho:Activity ;
    owl:equivalentClass [ a owl:Class ;
            owl:unionOf ( [ a owl:Restriction ;
                        owl:onProperty :hasEvent ;
                        owl:someValuesFrom [ a owl:Restriction ;
                                owl:hasValue ac:sleep ;
                                owl:onProperty :action ] ] [ a owl:Restriction ;
                        owl:onProperty :hasEvent ;
                        owl:someValuesFrom [ a owl:Restriction ;
                                owl:hasValue ac:wakeUp ;
                                owl:onProperty :action ] ] ) ] .

:Room a owl:Class ;
    rdfs:subClassOf :Object .

ho:Activity a owl:Class .

:Event a owl:Class ;
    skos:closeMatch <http://purl.org/NET/c4dm/event.owl#Event>,
        <http://semanticweb.cs.vu.nl/2009/11/sem/Event> .

x3do:Shape a owl:Class ;
    rdfs:comment "used for 3D bounding box" .

:Attribute a owl:Class .

ho:EatingDrinking a owl:Class ;
    rdfs:comment "Class that contains sequences for eating and drinking." ;
    rdfs:subClassOf ho:Activity ;
    owl:equivalentClass [ a owl:Class ;
            owl:unionOf ( [ a owl:Restriction ;
                        owl:onProperty :hasEvent ;
                        owl:someValuesFrom [ a owl:Restriction ;
                                owl:hasValue ac:drink ;
                                owl:onProperty :action ] ] [ a owl:Restriction ;
                        owl:onProperty :hasEvent ;
                        owl:someValuesFrom [ a owl:Restriction ;
                                owl:hasValue ac:eat ;
                                owl:onProperty :action ] ] ) ] .

:StateType a owl:Class .

ho:SocialInteraction a owl:Class ;
    rdfs:comment """Class that contains sequences that are related between , human-robot or \r
human-human interaction.""" ;
    rdfs:subClassOf ho:Activity .

ho:FoodPreparation a owl:Class ;
    rdfs:comment """Class for preparing food, or other kitchen based acitivities for eating \r
or drinking (prepeare coffee).""" ;
    rdfs:subClassOf ho:Activity .

ho:HouseCleaning a owl:Class ;
    rdfs:comment "The class that contains sequence of actions, with Cleaning tasks." ;
    rdfs:subClassOf ho:Activity .

ho:Leisure a owl:Class ;
    rdfs:comment "Class that contains procedures about leisure" ;
    rdfs:subClassOf ho:Activity .

ho:Work a owl:Class ;
    rdfs:comment "Class with related activites such as send an email, getting ready for work." ;
    rdfs:subClassOf ho:Activity .

ho:HygieneStyling a owl:Class ;
    rdfs:comment """Class for sequence that are related to Hygiene otr Styling (NOTICE: some \r
of this sequences could be conisdered also as cleaning).""" ;
    rdfs:subClassOf ho:Activity .

:Action a owl:Class .

ho:HouseArrangement a owl:Class ;
    rdfs:comment "Superclass that contains sequence for arrangement tasks inside the house. Some of these classes could have been classified as a House Cleaning subclass. We prefer this hierarchy, because the task are more to the category of organizing object inside a domestic environment, rather than cleaning." ;
    rdfs:subClassOf ho:Activity .

ho:Other a owl:Class ;
    rdfs:comment """This class contains instances that are tasks performed inside a domestic \r
envronmnet but could not be classified in a specific class.""" ;
    rdfs:subClassOf ho:Activity .

[] a owl:Axiom ;
    rdfs:comment "commented by vh2kg_ontology" ;
    owl:annotatedProperty rdfs:comment ;
    owl:annotatedSource x3do:Shape ;
    owl:annotatedTarget "used for 3D bounding box" .

[] a owl:AllDifferent ;
    owl:distinctMembers ( :bright :cold :dark :deep :heavy :high :hot :long :low :shallow :short :thick :thin ) .

